proof/definition_analysis/bn_base_proof.ec
@@ -1,0 +1,2652 @@
+require import AllCore IntDiv CoreMap List Distr.
+from Jasmin require import JModel_x86.
+import SLH64.
+
+require import JBigNum.
+
+
+
+abstract theory BN_base.
+
+op nlimbs : int.
+axiom gt0_nlimbs: 0 < nlimbs.
+
+clone import BN with
+  op nlimbs <- nlimbs
+  proof gt0_nlimbs by exact gt0_nlimbs.
+
+(*
+  extracted code from 'bn_base.jinc' with:
+  - 'nlimbs' turned a parameter;
+  - 'W64.t ArrayXX.t' turned 'BN.t'
+  - 'XX' in code turned 'nlimbs'
+  - removed parameterisation wrt 'SC:Systemcall_t"
+  - '__bn_rng" is "idealized"                 *  - 'bn_sample" is "idealized semantics of __bn_rsample"                 *)
+module M = {
+  proc __bn_load (a:W64.t) : BN.t = {
+    var aux: int;
+    
+    var x:BN.t;
+    var i:int;
+    var t:W64.t;
+    x <- witness;
+    i <- 0;
+    while (i < nlimbs) {
+      t <- (loadW64 Glob.mem (W64.to_uint (a + (W64.of_int (8 * i)))));
+      x.[i] <- t;
+      i <- i + 1;
+    }
+    return (x);
+  }
+  
+  proc __bn_store (a:W64.t, b:BN.t) : unit = {
+    var aux: int;
+    
+    var i:int;
+    var t:W64.t;
+    
+    i <- 0;
+    while (i < nlimbs) {
+      t <- b.[i];
+      Glob.mem <-
+      storeW64 Glob.mem (W64.to_uint (a + (W64.of_int (8 * i)))) (t);
+      i <- i + 1;
+    }
+    return ();
+  }
+  
+  proc __bn_eq_zf (a:BN.t, b:BN.t) : bool = {
+    var aux: int;
+    
+    var zf:bool;
+    var acc:W64.t;
+    var i:int;
+    var t:W64.t;
+    var  _0:bool;
+    var  _1:bool;
+    var  _2:bool;
+    var  _3:bool;
+    var  _4:W64.t;
+    
+    acc <- (W64.of_int 0);
+    i <- 0;
+    while (i < nlimbs) {
+      t <- a.[i];
+      t <- (t `^` b.[i]);
+      acc <- (acc `|` t);
+      i <- i + 1;
+    }
+    ( _0,  _1,  _2,  _3, zf,  _4) <- AND_64 acc acc;
+    return (zf);
+  }
+  
+  proc __bn_eq (a:BN.t, b:BN.t) : W64.t = {
+    
+    var res_0:W64.t;
+    var zf:bool;
+    var are_equal:W64.t;
+    
+    zf <@ __bn_eq_zf (a, b);
+    res_0 <- (W64.of_int 0);
+    are_equal <- (W64.of_int 1);
+    res_0 <- (zf ? are_equal : res_0);
+    return (res_0);
+  }
+  
+  proc _bn_eq (a:BN.t, b:BN.t) : W64.t = {
+    
+    var r:W64.t;
+    
+    r <@ __bn_eq (a, b);
+    return (r);
+  }
+  
+  proc _bn_eq_ (_a:BN.t, _b:BN.t) : W64.t = {
+    
+    var r:W64.t;
+    var a:BN.t;
+    var b:BN.t;
+    a <- witness;
+    b <- witness;
+    a <- _a;
+    b <- _b;
+    r <@ _bn_eq (a, b);
+    r <- r;
+    return (r);
+  }
+  
+  proc __bn_test0_zf (a:BN.t) : bool = {
+    var aux: int;
+    
+    var zf:bool;
+    var acc:W64.t;
+    var i:int;
+    var  _0:bool;
+    var  _1:bool;
+    var  _2:bool;
+    var  _3:bool;
+    var  _4:W64.t;
+    
+    acc <- a.[0];
+    i <- 1;
+    while (i < nlimbs) {
+      acc <- (acc `|` a.[i]);
+      i <- i + 1;
+    }
+    ( _0,  _1,  _2,  _3, zf,  _4) <- AND_64 acc acc;
+    return (zf);
+  }
+  
+  proc __bn_test0 (a:BN.t) : W64.t = {
+    
+    var res_0:W64.t;
+    var is_zero:W64.t;
+    var zf:bool;
+    
+    res_0 <- (W64.of_int 0);
+    is_zero <- (W64.of_int 1);
+    zf <@ __bn_test0_zf (a);
+    res_0 <- (zf ? is_zero : res_0);
+    return (res_0);
+  }
+  
+  proc _bn_test0 (a:BN.t) : W64.t = {
+    
+    var r:W64.t;
+    
+    r <@ __bn_test0 (a);
+    return (r);
+  }
+  
+  proc __bn_copy (a:BN.t) : BN.t = {
+    var aux: int;
+    
+    var r:BN.t;
+    var i:int;
+    var t:W64.t;
+    r <- witness;
+    i <- 0;
+    while (i < nlimbs) {
+      t <- a.[i];
+      r.[i] <- t;
+      i <- i + 1;
+    }
+    return (r);
+  }
+  
+  proc __bn_copy2 (a:BN.t, r:BN.t) : BN.t = {
+    var aux: int;
+    
+    var i:int;
+    var t:W64.t;
+    
+    i <- 0;
+    while (i < nlimbs) {
+      t <- a.[i];
+      r.[i] <- t;
+      i <- i + 1;
+    }
+    return (r);
+  }
+  
+  proc __bn_cmov (cond:bool, a:BN.t, b:BN.t) : 
+  BN.t = {
+    var aux: int;
+    
+    var i:int;
+    var t:W64.t;
+    
+    i <- 0;
+    while (i < nlimbs) {
+      t <- a.[i];
+      t <- (cond ? b.[i] : t);
+      a.[i] <- t;
+      i <- i + 1;
+    }
+    return (a);
+  }
+  
+  proc __bn_set0 (a:BN.t) : BN.t = {
+    var aux: int;
+    
+    var t:W64.t;
+    var i:int;
+    
+    t <- (W64.of_int 0);
+    i <- 0;
+    while (i < nlimbs) {
+      a.[i] <- t;
+      i <- i + 1;
+    }
+    return (a);
+  }
+  
+  proc __bn_add1c (a:BN.t, b:W64.t) : bool * BN.t = {
+    var aux: bool;
+    var aux_1: int;
+    var aux_0: W64.t;
+    
+    var cf:bool;
+    var i:int;
+    
+    (aux, aux_0) <- adc_64 a.[0] b false;
+    cf <- aux;
+    a.[0] <- aux_0;
+    i <- 1;
+    while (i < nlimbs) {
+      (aux, aux_0) <- adc_64 a.[i] (W64.of_int 0) cf;
+      cf <- aux;
+      a.[i] <- aux_0;
+      i <- i + 1;
+    }
+    return (cf, a);
+  }
+  
+  proc __bn_addc (a:BN.t, b:BN.t) : bool *
+                                                          BN.t = {
+    var aux: bool;
+    var aux_1: int;
+    var aux_0: W64.t;
+    
+    var cf:bool;
+    var t:W64.t;
+    var i:int;
+    
+    t <- b.[0];
+    (aux, aux_0) <- adc_64 a.[0] t false;
+    cf <- aux;
+    a.[0] <- aux_0;
+    i <- 1;
+    while (i < nlimbs) {
+      t <- b.[i];
+      (aux, aux_0) <- adc_64 a.[i] t cf;
+      cf <- aux;
+      a.[i] <- aux_0;
+      i <- i + 1;
+    }
+    return (cf, a);
+  }
+  
+  proc _bn_addc (a:BN.t, b:BN.t) : bool *
+                                                         BN.t = {
+    
+    var cf:bool;
+    
+    (cf, a) <@ __bn_addc (a, b);
+    return (cf, a);
+  }
+  
+  proc __bn_subc (a:BN.t, b:BN.t) : bool *
+                                                          BN.t = {
+    var aux: bool;
+    var aux_1: int;
+    var aux_0: W64.t;
+    
+    var cf:bool;
+    var t:W64.t;
+    var i:int;
+    
+    t <- b.[0];
+    (aux, aux_0) <- sbb_64 a.[0] t false;
+    cf <- aux;
+    a.[0] <- aux_0;
+    i <- 1;
+    while (i < nlimbs) {
+      t <- b.[i];
+      (aux, aux_0) <- sbb_64 a.[i] t cf;
+      cf <- aux;
+      a.[i] <- aux_0;
+      i <- i + 1;
+    }
+    return (cf, a);
+  }
+  
+  proc _bn_subc (a:BN.t, b:BN.t) : bool *
+                                                         BN.t = {
+    
+    var cf:bool;
+    
+    (cf, a) <@ __bn_subc (a, b);
+    return (cf, a);
+  }
+  
+  proc __bn_lt_cf (a:BN.t, b:BN.t) : bool = {
+    var aux: int;
+
+    var cf:bool;
+    var t:W64.t;
+    var i:int;
+
+    t <- a.[0];
+    (cf, t) <- sbb_64 t b.[0] false;
+    i <- 1;
+    while (i < nlimbs) {
+      t <- a.[i];
+      (cf, t) <- sbb_64 t b.[i] cf;
+      i <- i + 1;
+    }
+    return (cf);
+  }
+  
+  (* idealised version of randombytes *)
+  proc __bn_rnd (a:BN.t) : BN.t = {
+    a <$ BN.bn_rnd;
+    return a;
+  }
+  
+  (* idealised version of rsample *)
+  proc bn_sample_bnd (a:BN.t, bnd: BN.t) : BN.t = {
+    var i;
+    i <$ [0..bn bnd - 1];
+    a <- bn_ofint i;
+    return a;
+  }
+  
+  proc __bn_rsample (a:BN.t, bnd:BN.t) : BN.t = {
+    
+    var cf:bool;
+    
+    a <@ __bn_rnd (a);
+    cf <@ __bn_lt_cf (a, bnd);
+    while ((! cf)) {
+      a <@ __bn_rnd (a);
+      cf <@ __bn_lt_cf (a, bnd);
+    }
+    return (a);
+  }
+}.
+
+(** LOSSLESS lemmas *)
+lemma __bn_load_ll: islossless M.__bn_load.
+proof.
+proc; while (0 <= i <= nlimbs) (nlimbs - i).
+ by move=> z; auto => /> &m /#.
+by auto => />; smt(gt0_nlimbs).
+qed.
+
+lemma __bn_store_ll: islossless M.__bn_store.
+proof.
+proc; while (0 <= i <= nlimbs) (nlimbs - i).
+ by move=> z; auto => /> &m /#.
+by auto => />; smt(gt0_nlimbs).
+qed.
+
+lemma __bn_eq_zf_ll: islossless M.__bn_eq_zf.
+proof.
+proc; wp; while (0 <= i <= nlimbs) (nlimbs - i).
+ by move=> z; auto => /> &m /#.
+by auto => />; smt(gt0_nlimbs).
+qed.
+
+lemma __bn_eq_ll: islossless M.__bn_eq.
+proof. by proc; wp; call __bn_eq_zf_ll. qed.
+
+lemma _bn_eq_ll: islossless M._bn_eq.
+proof. by proc; call __bn_eq_ll. qed.
+
+lemma _bn_eq__ll: islossless M._bn_eq_.
+proof. by proc; wp; call _bn_eq_ll; auto. qed.
+
+lemma __bn_test0_zf_ll: islossless M.__bn_test0_zf.
+proof.
+proc; wp; while (0 <= i <= nlimbs) (nlimbs - i).
+ by move=> z; auto => /> &m /#.
+by auto => />; smt(gt0_nlimbs).
+qed.
+
+lemma __bn_test0_ll: islossless M.__bn_test0.
+proof. by proc; wp; call __bn_test0_zf_ll; auto. qed.
+
+lemma _bn_test0_ll: islossless M._bn_test0.
+proof. by proc; call __bn_test0_ll. qed.
+
+lemma __bn_copy_ll: islossless M.__bn_copy.
+proof.
+proc; wp; while (0 <= i <= nlimbs) (nlimbs - i).
+ by move=> z; auto => /> &m /#.
+by auto => />; smt(gt0_nlimbs).
+qed.
+
+lemma __bn_copy2_ll: islossless M.__bn_copy2.
+proof.
+proc; wp; while (0 <= i <= nlimbs) (nlimbs - i).
+ by move=> z; auto => /> &m /#.
+by auto => />; smt(gt0_nlimbs).
+qed.
+
+lemma __bn_cmov_ll: islossless M.__bn_cmov.
+proof.
+proc; wp; while (0 <= i <= nlimbs) (nlimbs - i).
+ by move=> z; auto => /> &m /#.
+by auto => />; smt(gt0_nlimbs).
+qed.
+
+lemma __bn_set0_ll: islossless M.__bn_set0.
+proof.
+proc; while (0 <= i <= nlimbs) (nlimbs - i).
+ by move=> z; auto => /> &m /#.
+by auto => />; smt(gt0_nlimbs).
+qed.
+
+lemma __bn_add1c_ll: islossless M.__bn_add1c.
+proof.
+proc; while (0 <= i <= nlimbs) (nlimbs - i).
+ by move=> z; auto => /> &m /#.
+by auto => />; smt(gt0_nlimbs).
+qed.
+
+lemma __bn_addc_ll: islossless M.__bn_addc.
+proof.
+proc; while (0 <= i <= nlimbs) (nlimbs - i).
+ by move=> z; auto => /> &m /#.
+by auto => />; smt(gt0_nlimbs).
+qed.
+
+lemma _bn_addc_ll: islossless M._bn_addc.
+proof. by proc; call __bn_addc_ll. qed.
+
+lemma __bn_subc_ll: islossless M.__bn_subc.
+proof.
+proc; while (0 <= i <= nlimbs) (nlimbs - i).
+ by move=> z; auto => /> &m /#.
+by auto => />; smt(gt0_nlimbs).
+qed.
+
+lemma __bn_lt_cf_ll: islossless M.__bn_lt_cf.
+proof.
+proc; while (0 <= i <= nlimbs) (nlimbs - i).
+ by move=> z; auto => /> &m /#.
+by auto => />; smt(gt0_nlimbs).
+qed.
+
+lemma _bn_subc_ll: islossless M._bn_subc.
+proof. by proc; call __bn_subc_ll. qed.
+
+(* Correctness lemmas *)
+
+hoare __bn_eq_zf_h _a _b:
+ M.__bn_eq_zf: a=_a /\ b=_b ==> res =  (_a=_b).
+proof.
+proc; simplify. 
+wp; while ( #pre /\ 0 <= i <= nlimbs /\ ((acc = W64.zero) <=> (bnk i a = bnk i b))).
+ wp; skip => /> &hr Hi1 Hi2 [HL HR] Hi3.
+ split; first smt().
+ split.
+  rewrite orw_eq0 xorw_eq0; move => [E1 E2].
+  by rewrite !bnkS 1..2:/# /= E2 (HL E1) /#.
+ move => /(bnkS_eq _ _ _ Hi1) [E1 E2].
+ by rewrite orw_eq0 (HR E2) E1.
+wp; skip => />; split; first smt(gt0_nlimbs bnk0).
+move=> acc i ???; rewrite (_:i=nlimbs) 1:/#.
+move=> [H1 H2].
+rewrite /AND_64 /rflags_of_bwop_w /flags_w /rflags_of_bwop /ZF_of /=.
+by case: (acc = W64.zero) => C; smt(bn_inj).
+qed.
+
+phoare __bn_eq_zf_ph _a _b:
+ [M.__bn_eq_zf: a=_a /\ b=_b ==> res = (_a=_b)] = 1%r.
+proof. by conseq __bn_eq_zf_ll (__bn_eq_zf_h _a _b). qed.
+
+hoare __bn_eq_h _a _b:
+ M.__bn_eq: a=_a /\ b=_b ==> to_uint res =  b2i (_a=_b).
+proof.
+proc; wp; call (__bn_eq_zf_h _a _b); skip => />.
+by case: (_a=_b) => C /#.
+qed.
+
+phoare __bn_eq_ph _a _b:
+ [M.__bn_eq: a=_a /\ b=_b ==> to_uint res =  b2i (_a=_b)] = 1%r.
+proof. by conseq __bn_eq_ll (__bn_eq_h _a _b). qed.
+
+hoare _bn_eq_h _a _b:
+ M._bn_eq: a=_a /\ b=_b ==> to_uint res = b2i (_a=_b).
+proof. by proc; ecall (__bn_eq_h a b). qed.
+
+phoare _bn_eq_ph _a _b:
+ [M._bn_eq: a=_a /\ b=_b ==> to_uint res = b2i (_a=_b)] = 1%r.
+proof. by conseq _bn_eq_ll (_bn_eq_h _a _b). qed.
+ 
+hoare _bn_eq__h a b:
+ M._bn_eq_: _a=a /\ _b=b ==> to_uint res = b2i (a=b).
+proof. by proc; wp; ecall (_bn_eq_h a b); auto. qed.
+ 
+phoare _bn_eq__ph a b:
+ [M._bn_eq_: _a=a /\ _b=b ==> to_uint res = b2i (a=b) ] = 1%r.
+proof. by conseq _bn_eq__ll (_bn_eq__h a b). qed.
+
+hoare __bn_test0_zf_h _a:
+ M.__bn_test0_zf: a=_a ==> res = (bn _a=0).
+proof.
+proc.
+wp; while ( #pre /\ 0 <= i <= nlimbs /\ ((acc = W64.zero) <=> (bnk i a = 0))).
+ wp; skip; progress; first 2 smt().
+  move: H3; rewrite orw_eq0 => [[E1 E2]].
+  by rewrite bnkS 1:/# /= E2 to_uint0 /= -H1 E1.
+ move: (bnkS_eq0 _ _ H H3) => {H3} [H31 H32].
+ by rewrite orw_eq0 H1 H32 /= to_uint_eq /#.
+wp; skip => />; progress.
+   smt(gt0_nlimbs).
+  by rewrite bnk1 /= H to_uint0.
+ by move: H; rewrite bnk1 /= to_uint_eq /=.
+move: H2; rewrite (_:i0=nlimbs) 1:/# => <-.
+by rewrite /AND_64 /#.
+qed.
+
+phoare __bn_test0_zf_ph _a:
+ [M.__bn_test0_zf: a=_a ==> res = (bn _a=0)] = 1%r.
+proof. by conseq __bn_test0_zf_ll (__bn_test0_zf_h _a). qed.
+
+hoare __bn_test0_h _a:
+ M.__bn_test0: a=_a ==> to_uint res = b2i (bn _a=0).
+proof.
+proc; wp; call (__bn_test0_zf_h _a); auto => />.
+case (bnk nlimbs _a = 0) => _; smt().
+qed.
+
+phoare __bn_test0_ph _a:
+ [M.__bn_test0: a=_a ==> to_uint res = b2i (bn _a=0)] = 1%r.
+proof. by conseq __bn_test0_ll (__bn_test0_h _a). qed.
+
+hoare _bn_test0_h _a:
+ M._bn_test0: a=_a ==> to_uint res = b2i (bn _a=0).
+proof. by proc; ecall (__bn_test0_h a). qed.
+ 
+phoare _bn_test0_ph _a:
+ [M._bn_test0: a=_a ==> to_uint res = b2i (bn _a=0)] = 1%r.
+proof. by conseq _bn_test0_ll (_bn_test0_h _a). qed.
+
+hoare __bn_copy_h _a:
+ M.__bn_copy: a=_a ==> res = _a.
+proof.
+proc; while (0 <= i <= nlimbs /\ _a = a /\ (forall j, 0 <= j < i => r.[j] = _a.[j])).
+ by wp; skip; progress; [smt() | smt() | rewrite get_setE => /#]. 
+wp; skip; progress; first 2 smt(gt0_nlimbs).  
+by rewrite tP /#.
+qed.
+
+phoare __bn_copy_ph _a:
+ [M.__bn_copy: a=_a ==> res = _a] = 1%r.
+proof. by conseq __bn_copy_ll (__bn_copy_h _a). qed.
+
+hoare __bn_copy2_h _a:
+ M.__bn_copy2: a=_a ==> res = _a.
+proof.
+proc; while (0 <= i <= nlimbs /\ _a = a /\ (forall j, 0 <= j < i => r.[j] = _a.[j])).
+ by wp; skip; progress; [smt() | smt() | rewrite get_setE => /#]. 
+wp; skip; progress; first 2 smt(gt0_nlimbs).  
+by rewrite tP /#.
+qed.
+
+phoare __bn_copy2_ph _a:
+ [M.__bn_copy2: a=_a ==> res = _a] = 1%r.
+proof. by conseq __bn_copy2_ll (__bn_copy2_h _a). qed.
+
+hoare __bn_cmov_h _cond _a _b:
+ M.__bn_cmov: cond=_cond /\ a=_a /\ b=_b
+              ==> res = if _cond then _b else _a.
+proof.
+proc => //=. 
+while (0 <= i <= nlimbs /\ _cond = cond /\ _b = b /\
+       (forall j, i <= j < nlimbs => a.[j] = _a.[j]) /\
+       forall j, 0 <= j < i => a.[j] = if _cond then _b.[j] else _a.[j]).
+ wp; skip => /> &hr *; split; first smt().
+ split.
+  move=> j Hj1 Hj2; rewrite get_setE 1:/#.
+  by rewrite ifF 1:/# /#.
+ by move=> j Hj1 Hj2; rewrite get_setE 1:/# /#.
+wp; skip => />. split; first smt(gt0_nlimbs).
+move=> a i ???; rewrite (:i=nlimbs) 1:/# => H1 H2.
+by rewrite tP /#.
+qed.
+
+phoare __bn_cmov_ph _cond _a _b:
+ [M.__bn_cmov: cond=_cond /\ a=_a /\ b=_b
+              ==> res = if _cond then _b else _a] = 1%r.
+proof. by conseq __bn_cmov_ll (__bn_cmov_h _cond _a _b). qed.
+
+hoare __bn_set0_h:
+ M.__bn_set0 : true ==> bn res = 0.
+proof.
+proc.
+while (bnk i a = 0 /\ 0 <= i <= nlimbs /\ to_uint t = 0).
+ auto => /> *.
+ by rewrite bnkS 1:/# /= get_setE 1:/# bnk_setO /#.
+by auto => /> &m; smt(bnk0 gt0_nlimbs).
+qed.
+
+phoare __bn_set0_ph:
+ [M.__bn_set0 : true ==> bn res = 0] = 1%r.
+proof. by conseq __bn_set0_ll __bn_set0_h. qed.
+
+(* bnk with carry *)
+op bnk_withcarry k (x: bool * t): int =
+ b2i x.`1 * W64.modulus ^ k + bnk k x.`2. 
+
+abbrev bn_withcarry x = bnk_withcarry nlimbs x.
+
+op bnk_addc k cf (a:t) x = 
+ ((addc a.[k] x cf).`1, a.[k <- (addc a.[k] x cf).`2]).
+
+op to_uint_withcarry (cw:bool*W64.t) =
+ W64.to_uint cw.`2 + b2i cw.`1 * W64.modulus.
+
+lemma to_uint_withcarry_addc x y cf:
+ to_uint_withcarry (W64.addc x y cf)
+ = to_uint x + to_uint y + b2i cf.
+proof.
+move: (W64.addcP x y cf) => /=.
+by rewrite /to_uint_withcarry mulrC addcE /=.
+qed.
+
+lemma bnk_withcarryS k cf a x:
+ 0 <= k < nlimbs =>
+ bnk_withcarry (k+1) (bnk_addc k cf a x)
+ = (to_uint a.[k] + to_uint x) * W64.modulus ^ k
+   + bnk_withcarry k (cf,a).
+proof.
+move=> Hk; rewrite /bnk_withcarry /bnk_addc /= bnkS 1:/# addcE /= bnk_setO 1:/# get_setE 1:/# /=.
+move: (W64.addcP a.[k] x cf); rewrite addcE /= => E.
+rewrite exprS 1:/#; ring E.
+qed.
+
+hoare __bn_add1c_h _a _b:
+ M.__bn_add1c :
+ a=_a /\ b=_b
+ ==> bn_withcarry res = bn _a + to_uint _b.
+proof.
+have Hlimbs:= gt0_nlimbs; proc; simplify.
+while (1 <= i <= nlimbs /\ _b = b /\
+       (forall j, i <= j < nlimbs => a.[j] = _a.[j]) /\
+       bnk_withcarry i (cf, a) = bnk i _a + to_uint b).
+ wp; skip => &hr [[[Hi1 Hi2]]] /> Ha H Hc.
+ split; [smt() | split].
+  by move=> j Hj1 Hj2; rewrite get_setE 1:/# ifF /#.
+ rewrite -/(bnk_addc i{hr} cf{hr} a{hr} W64.zero).
+ rewrite bnk_withcarryS 1:/# bnkS 1:/# /=. 
+ by rewrite -addzA -H /#.
+auto => />; split.
+ split; first smt().
+ split.
+  by move=> j Hj1 Hj2; rewrite get_setE /#.
+ rewrite -/(bnk_addc 0 false _a _b).
+ rewrite {1}(:1=0+1) 1:/# bnk_withcarryS 1:/# expr0 bnk1 /=.
+ by rewrite /bnk_withcarry /= b2i0 bnk0 /=.
+by move=> a cf i ??? _; rewrite (:i=nlimbs) 1:/#.
+qed.
+
+(*
+get_setE 1:/# bnk_setO 1:/# /=.
+print addcE.
+  by rewrite addcE !bn_carryS /= 1:/# carryE /carry_add /= bn_digitS // to_uint0 /=.
+ rewrite !bnkS /= 1..2:/# get_setE 1:/# /= bnk_setO 1:/# H1.
+ by rewrite addcP' !exprS 1:/# carryE addcE /carry_add /=; ring.
+wp; skip => /> .
+split.
+ split; first by smt().
+ split.
+  by rewrite (_: 1 = 0 + 1) // bn_carryS // bn_carry0 bn_digit0 carryE addcE /= /carry_add.
+ rewrite (_: 1 = 0 + 1) // !bnkS //= !bnk0 //= get_setE 1:/# //=.
+ by rewrite addcP' addcE carryE /carry_add /=.
+move => j dd Hj1 Hj2 Hj3 Hwsize; split.
+ by rewrite (_ : j = nlimbs) 1:/# bn_carryE 1:/# bn_modulusE bn_digit.
+move: Hwsize; rewrite (_:j = nlimbs) 1:/# => ->.
+have Hwsize:= W64.ge0_size.
+pose X:= (bn_carry _ _ _ _); case: X; rewrite /X => {X} H.
+ rewrite b2i1 -(modzMDr (-1)) bn_modulusE /= modz_small.
+  rewrite ger0_norm; first smt(expr_gt0).
+  have ->/=: bnk nlimbs aa + to_uint bb + b2i cc + (-1) * W64.modulus ^ nlimbs = bnk nlimbs aa + to_uint bb + b2i cc + -1 * W64.modulus ^ nlimbs by smt().
+  apply mod_sub.
+  - by smt(expr_gt0).
+  - by move: bnk_cmp; smt().
+  - split => *; first smt(to_uint_cmp).
+    by move: to_uint_cmp ler_eexpr; smt().
+  - by move: H; rewrite bn_carryE 1:/# bn_digit /#.
+ by smt().
+rewrite b2i0 bn_modulusE -exprM /=.
+move: H; rewrite /X bn_carryE 1:/# => H.
+rewrite modz_small // ger0_norm; first smt(expr_gt0).
+split => *; first move: to_uint_cmp bnk_cmp; smt().
+by rewrite exprM; rewrite bn_digit -ltzNge in H.
+
+qed.
+*)
+
+phoare __bn_add1c_ph _a _b:
+ [ M.__bn_add1c :
+   a=_a /\ b=_b
+   ==> bn_withcarry res = bn _a + to_uint _b] = 1%r.
+proof. by conseq __bn_add1c_ll (__bn_add1c_h _a _b). qed.
+
+hoare __bn_addc_h _a _b:
+ M.__bn_addc : 
+ a=_a /\ b=_b ==> bn_withcarry res = bn _a + bn _b.
+proof.
+have Hlimbs:= gt0_nlimbs; proc; simplify.
+while (1 <= i <= nlimbs /\ _b = b /\
+       (forall j, i <= j < nlimbs => a.[j] = _a.[j]) /\
+       bnk_withcarry i (cf, a) = bnk i _a + bnk i _b).
+ wp; skip => &hr [[[Hi1 Hi2]]] /> Ha H Hc.
+ split; [smt() | split].
+  by move=> j Hj1 Hj2; rewrite get_setE 1:/# ifF /#.
+ rewrite -/(bnk_addc i{hr} cf{hr} a{hr} b{hr}.[i{hr}]).
+ rewrite bnk_withcarryS 1:/# !bnkS 1..2:/# /=.
+ rewrite Ha 1:/#. 
+ by ring H.
+auto => />; split.
+ split; first smt().
+ split.
+  by move=> j Hj1 Hj2; rewrite get_setE /#.
+ rewrite -/(bnk_addc 0 false _a _b.[0]).
+ rewrite {1}(:1=0+1) 1:/# bnk_withcarryS 1:/# expr0 !bnk1 /=.
+ by rewrite /bnk_withcarry /= b2i0 bnk0 /=.
+by move=> a cf i ??? _; rewrite (:i=nlimbs) 1:/#.
+qed.
+
+phoare __bn_addc_ph _a _b:
+ [ M.__bn_addc : 
+   a=_a /\ b=_b 
+   ==> bn_withcarry res = bn _a + bn _b] = 1%r.
+proof. by conseq __bn_addc_ll (__bn_addc_h _a _b). qed.
+
+hoare _bn_addc_h _a _b:
+ M._bn_addc : 
+ a=_a /\ b=_b
+ ==> bn_withcarry res = bn _a + bn _b.
+proof. by proc; ecall (__bn_addc_h a b). qed.
+
+phoare _bn_addc_ph _a _b:
+ [ M._bn_addc : 
+   a=_a /\ b=_b 
+   ==> bn_withcarry res = bn _a + bn _b] = 1%r.
+proof. by conseq _bn_addc_ll (_bn_addc_h _a _b). qed.
+
+(* bn with borrow *)
+op bnk_withborrow k (x: bool * t): int =
+ bnk k x.`2 - b2i x.`1 * W64.modulus ^ k.
+
+abbrev bn_withborrow x = bnk_withborrow nlimbs x.
+(*
+op bnb (x: bool * t): int = bn x.`2 - b2i x.`1 * bn_modulus. 
+*)
+op bnk_subc k cf (a:t) x = 
+ ((subc a.[k] x cf).`1, a.[k <- (subc a.[k] x cf).`2]).
+
+op to_uint_withborrow (cw:bool*W64.t) =
+ W64.to_uint cw.`2 - b2i cw.`1 * W64.modulus.
+
+lemma to_uint_withborrow_subc x y cf:
+ to_uint_withborrow (W64.subc x y cf)
+ = to_uint x - (to_uint y + b2i cf).
+proof.
+move: (W64.subcP x y cf) => /=.
+by rewrite /to_uint_withborrow mulrC subcE /=.
+qed.
+
+lemma bnk_withborrowS k cf a x:
+ 0 <= k < nlimbs =>
+ bnk_withborrow (k+1) (bnk_subc k cf a x)
+ = (to_uint a.[k] - to_uint x) * W64.modulus ^ k
+   + bnk_withborrow k (cf,a).
+proof.
+move=> Hk; rewrite /bnk_withborrow /bnk_subc /= bnkS 1:/# subcE /= bnk_setO 1:/# get_setE 1:/# /=.
+move: (W64.subcP a.[k] x cf); rewrite subcE /= => E.
+rewrite exprS 1:/#; ring E.
+qed.
+
+
+hoare __bn_subc_h _a _b:
+ M.__bn_subc :
+ a=_a /\ b=_b 
+ ==> bn_withborrow res = bn _a - bn _b.
+proof.
+have Hlimbs:= gt0_nlimbs; proc; simplify.
+while (1 <= i <= nlimbs /\ _b = b /\
+       (forall j, i <= j < nlimbs => a.[j] = _a.[j]) /\
+       bnk_withborrow i (cf, a) = bnk i _a - bnk i _b).
+ wp; skip => &hr [[[Hi1 Hi2]]] /> Ha H Hc.
+ split; [smt() | split].
+  by move=> j Hj1 Hj2; rewrite get_setE 1:/# ifF /#.
+ rewrite -/(bnk_subc i{hr} cf{hr} a{hr} b{hr}.[i{hr}]).
+ rewrite bnk_withborrowS 1:/# !bnkS 1..2:/# /=.
+ rewrite Ha 1:/#. 
+ by ring H.
+auto => />; split.
+ split; first smt().
+ split.
+  by move=> j Hj1 Hj2; rewrite get_setE /#.
+ rewrite -/(bnk_subc 0 false _a _b.[0]).
+ rewrite {1}(:1=0+1) 1:/# bnk_withborrowS 1:/# expr0 !bnk1 /=.
+ by rewrite /bnk_withborrow /= b2i0 bnk0 /=.
+by move=> a cf i ??? _; rewrite (:i=nlimbs) 1:/#.
+qed.
+
+phoare __bn_subc_ph _a _b:
+ [ M.__bn_subc :
+   a=_a /\ b=_b 
+   ==> bn_withborrow res = bn _a - bn _b] = 1%r.
+proof. by conseq __bn_subc_ll (__bn_subc_h _a _b). qed.
+
+hoare __bn_lt_cf_h _a _b:
+ M.__bn_lt_cf : a=_a /\ b=_b ==> res = bn _a < bn _b.
+proof.
+have Hlimbs:= gt0_nlimbs; proc; simplify.
+while (1 <= i <= nlimbs /\ _a = a /\ _b = b /\
+       cf = (bnk i _a < bnk i _b)).
+ wp; skip => &hr [[[Hi1 _]]] /> Hi.
+ split; [smt() |].
+ rewrite subcE /borrow_sub /=.
+ rewrite (bnk_ltb i{hr} a{hr} b{hr} false _) 1:/#.
+ case: (bnk i{hr} a{hr} < bnk i{hr} b{hr}) => C.
+  by rewrite b2i1 b2i0 C /= ltzS StdOrder.IntOrder.ler_eqVlt to_uint_eq /#.
+ by rewrite b2i0 /#.
+auto => />; split.
+ split; first smt().
+ by rewrite subcE /borrow_sub b2i0 /= !bnk1.
+by move=> i ???; rewrite (:i=nlimbs) 1:/#.
+qed.
+
+phoare __bn_lt_cf_ph _a _b:
+ [M.__bn_lt_cf : a=_a /\ b=_b ==> res = bn _a < bn _b] = 1%r.
+proof. by conseq __bn_lt_cf_ll (__bn_lt_cf_h _a _b). qed.
+
+
+(* REJECTION SAMPLING *)
+
+phoare __bn_rnd_ph _res:
+ [ M.__bn_rnd :
+   true ==> res = _res ] = (mu1 bn_rnd _res).
+proof. by proc; rnd; skip => />. qed.
+
+phoare bn_sample_bnd_ph _bnd _res:
+ [ M.bn_sample_bnd :
+   bnd=_bnd ==> res = _res ] = (mu1 (bn_rnd_bnd bnd) _res).
+proof. 
+proc; wp; rnd; skip => />. 
+by rewrite dmap1E /pred1 /(\o) /=.
+qed.
+
+require import DInterval Dexcepted.
+clone import WhileSampling as RS
+ with type input = unit,
+      type t = BN.t,
+      op dt i = bn_rnd.
+
+equiv __bn_rsample_eq:
+ M.__bn_rsample ~ M.bn_sample_bnd :
+ ={bnd} ==> ={res}.
+proof.
+exlim bnd{2} => _bnd.
+case: (bn _bnd = 0) => Hbnd.
+ bypr res{1} res{2} => //.
+ move=> &1 &2 _a [Hbnd1 Hbnd2].
+ pose P:= Pr[M.bn_sample_bnd(_, _) @ &2 : res = _].
+ have ->: P = 0%r.
+  rewrite /P; byphoare (: bnd=bnd{2} ==> _) => //; hoare.
+  by proc; auto => /> i; rewrite supp_dinter; smt(bnk_cmp).
+ byphoare (: bnd=_bnd ==> _) => //.
+  hoare; proc; while(bnd=_bnd /\ cf = bnk nlimbs a < bnk nlimbs _bnd).
+   ecall (__bn_lt_cf_h a bnd).
+   by inline*; auto => /> &m.
+  ecall (__bn_lt_cf_h a bnd).
+  inline*; auto => &m -> a Ha r; rewrite Hbnd.
+  smt(bnk_cmp).
+ smt().
+transitivity
+ RS.SampleW.sample
+ (bnd{1}=_bnd /\ i{2}=tt /\ test{2}=fun _ n =>! bn n < bn _bnd
+  ==> ={res})
+ (bnd{2}=_bnd /\ i{1}=tt /\ test{1}=fun _ n =>! bn n < bn _bnd
+  ==> ={res}) => //=.
++ move=> &1 &2 [E E2].
+  by exists (tt,fun _ n => !bn n < bn _bnd) => /#.
++ proc; simplify; inline SampleWi.sample.
+  wp; while (#pre /\ test0{2}=test{2} /\ a{1}=r0{2} /\
+             (!cf{1})=(test0 i0 r0){2}).
+   ecall {1} (__bn_lt_cf_ph a{1} bnd{1}).
+   by inline*; auto => />.
+  ecall {1} (__bn_lt_cf_ph a{1} bnd{1}).
+  by inline*; auto => &1 &2 /=.
+transitivity RS.SampleE.sample
+ (={i,test} /\ i{2}=tt /\ test{2}=fun _ n =>! bn n < bn _bnd
+  ==> ={res})
+ (bnd{2}=_bnd /\ i{1}=tt /\ test{1}=fun _ n =>! bn n < bn _bnd
+  ==> ={res}) => //=.
++ move=> &1 &2 [E2 E].
+  by exists (tt,fun _ n => !bn n < bn _bnd) => /#.
++ symmetry; conseq RS.sampleE_sampleW.
+   by move => /> &1 &2 -> _ /=; apply bn_rnd_ll.
+  by move=> />.
+proc; simplify.
+rnd : 0 *0; skip => /> &1; split.
+ move=> a; rewrite supp_dmap => [[i />]].
+ rewrite supp_dinter => Hi.
+ rewrite !dmap1E /pred1 /(\o) /=.
+ rewrite bn_rnd_excepted dmapE.
+ apply mu_eq_support.
+ by move=> x; rewrite supp_dinter /(\o) /=.
+move => H1 r /=.
+rewrite supp_dmap => [[a />]].
+rewrite supp_dexcepted /= => [[HA HB]].
+rewrite supp_dmap; exists (bn a); split.
+ by rewrite supp_dinter; smt(bnk_cmp).
+by rewrite bnK.
+qed.
+
+phoare __bn_rsample_ph _bnd _res:
+ [ M.__bn_rsample :
+   bnd=_bnd ==> res = _res ] = (mu1 (bn_rnd_bnd bnd) _res).
+proof.
+conseq __bn_rsample_eq (bn_sample_bnd_ph _bnd _res) => /> &1.
+by exists (bnd{1},bnd{1}); smt().
+qed.
+
+lemma bn_sample_bnd_ll:
+ phoare [ M.bn_sample_bnd : 0 < bn bnd ==> true ] = 1%r.
+proof.
+proc; simplify; auto => /> &m Hbnd.
+by rewrite weight_dinter /#.
+qed.
+
+lemma __bn_rsample_ll:
+ phoare [ M.__bn_rsample : 0 < bn bnd ==> true ] = 1%r.
+proof.
+conseq __bn_rsample_eq bn_sample_bnd_ll => //=.
+by move=> /> &1 Hbnd; exists (witness, bnd{1}) => /#.
+qed.
+
+
+
+
+from Jasmin require import JLeakage.
+
+module Mleak = {
+  var leakages : leakages_t
+
+  proc __bn_load (a:W64.t) : BN.t = {
+    var aux: int;
+    var aux_0: W64.t;
+    
+    var x:BN.t;
+    var i:int;
+    var t:W64.t;
+    x <- witness;
+    leakages <- LeakFor(0,nlimbs) :: LeakAddr([]) :: leakages;
+    i <- 0;
+    while (i < nlimbs) {
+      leakages <- LeakAddr([(W64.to_uint (a + (W64.of_int (8 * i))))]) :: leakages;
+      aux_0 <- (loadW64 Glob.mem (W64.to_uint (a + (W64.of_int (8 * i)))));
+      t <- aux_0;
+      leakages <- LeakAddr([]) :: leakages;
+      aux_0 <- t;
+      leakages <- LeakAddr([i]) :: leakages;
+      x.[i] <- aux_0;
+      i <- i + 1;
+    }
+    return (x);
+  }
+  
+  proc __bn_store (a:W64.t, b:BN.t) : unit = {
+    var aux: int;
+    var aux_0: W64.t;
+    
+    var i:int;
+    var t:W64.t;
+    
+    leakages <- LeakFor(0,nlimbs) :: LeakAddr([]) :: leakages;
+    i <- 0;
+    while (i < nlimbs) {
+      leakages <- LeakAddr([i]) :: leakages;
+      aux_0 <- b.[i];
+      t <- aux_0;
+      leakages <- LeakAddr([]) :: leakages;
+      aux_0 <- t;
+      leakages <- LeakAddr([(W64.to_uint (a + (W64.of_int (8 * i))))]) :: leakages;
+      Glob.mem <-
+      storeW64 Glob.mem (W64.to_uint (a + (W64.of_int (8 * i)))) (aux_0);
+      i <- i + 1;
+    }
+    return ();
+  }
+  
+  proc __bn_eq_zf (a:BN.t, b:BN.t) : bool = {
+    var aux_5: bool;
+    var aux_4: bool;
+    var aux_3: bool;
+    var aux_2: bool;
+    var aux_1: bool;
+    var aux_0: int;
+    var aux: W64.t;
+    
+    var zf:bool;
+    var acc:W64.t;
+    var i:int;
+    var t:W64.t;
+    var  _0:bool;
+    var  _1:bool;
+    var  _2:bool;
+    var  _3:bool;
+    var  _4:W64.t;
+    
+    leakages <- LeakAddr([]) :: leakages;
+    aux <- (W64.of_int 0);
+    acc <- aux;
+    leakages <- LeakFor(0,nlimbs) :: LeakAddr([]) :: leakages;
+    i <- 0;
+    while (i < nlimbs) {
+      leakages <- LeakAddr([i]) :: leakages;
+      aux <- a.[i];
+      t <- aux;
+      leakages <- LeakAddr([i]) :: leakages;
+      aux <- (t `^` b.[i]);
+      t <- aux;
+      leakages <- LeakAddr([]) :: leakages;
+      aux <- (acc `|` t);
+      acc <- aux;
+      i <- i + 1;
+    }
+    leakages <- LeakAddr([]) :: leakages;
+    (aux_5, aux_4, aux_3, aux_2, aux_1, aux) <- AND_64 acc acc;
+     _0 <- aux_5;
+     _1 <- aux_4;
+     _2 <- aux_3;
+     _3 <- aux_2;
+    zf <- aux_1;
+     _4 <- aux;
+    return (zf);
+  }
+  
+  proc __bn_eq (a:BN.t, b:BN.t) : W64.t = {
+    var aux: bool;
+    var aux_0: W64.t;
+    
+    var res_0:W64.t;
+    var zf:bool;
+    var are_equal:W64.t;
+    
+    leakages <- LeakAddr([]) :: leakages;
+    aux <@ __bn_eq_zf (a, b);
+    zf <- aux;
+    leakages <- LeakAddr([]) :: leakages;
+    aux_0 <- (W64.of_int 0);
+    res_0 <- aux_0;
+    leakages <- LeakAddr([]) :: leakages;
+    aux_0 <- (W64.of_int 1);
+    are_equal <- aux_0;
+    leakages <- LeakAddr([]) :: leakages;
+    aux_0 <- (zf ? are_equal : res_0);
+    res_0 <- aux_0;
+    return (res_0);
+  }
+  
+  proc _bn_eq (a:BN.t, b:BN.t) : W64.t = {
+    var aux: W64.t;
+    
+    var r:W64.t;
+    
+    leakages <- LeakAddr([]) :: leakages;
+    aux <@ __bn_eq (a, b);
+    r <- aux;
+    return (r);
+  }
+  
+  proc _bn_eq_ (_a:BN.t, _b:BN.t) : W64.t = {
+    var aux_0: W64.t;
+    var aux: BN.t;
+    
+    var r:W64.t;
+    var a:BN.t;
+    var b:BN.t;
+    a <- witness;
+    b <- witness;
+    leakages <- LeakAddr([]) :: leakages;
+    aux <- _a;
+    a <- aux;
+    leakages <- LeakAddr([]) :: leakages;
+    aux <- _b;
+    b <- aux;
+    leakages <- LeakAddr([]) :: leakages;
+    aux_0 <@ _bn_eq (a, b);
+    r <- aux_0;
+    leakages <- LeakAddr([]) :: leakages;
+    aux_0 <- r;
+    r <- aux_0;
+    return (r);
+  }
+  
+  proc __bn_test0_zf (a:BN.t) : bool = {
+    var aux_5: bool;
+    var aux_4: bool;
+    var aux_3: bool;
+    var aux_2: bool;
+    var aux_1: bool;
+    var aux_0: int;
+    var aux: W64.t;
+    
+    var zf:bool;
+    var acc:W64.t;
+    var i:int;
+    var  _0:bool;
+    var  _1:bool;
+    var  _2:bool;
+    var  _3:bool;
+    var  _4:W64.t;
+    
+    leakages <- LeakAddr([0]) :: leakages;
+    aux <- a.[0];
+    acc <- aux;
+    leakages <- LeakFor(1,nlimbs) :: LeakAddr([]) :: leakages;
+    i <- 1;
+    while (i < nlimbs) {
+      leakages <- LeakAddr([i]) :: leakages;
+      aux <- (acc `|` a.[i]);
+      acc <- aux;
+      i <- i + 1;
+    }
+    leakages <- LeakAddr([]) :: leakages;
+    (aux_5, aux_4, aux_3, aux_2, aux_1, aux) <- AND_64 acc acc;
+     _0 <- aux_5;
+     _1 <- aux_4;
+     _2 <- aux_3;
+     _3 <- aux_2;
+    zf <- aux_1;
+     _4 <- aux;
+    return (zf);
+  }
+  
+  proc __bn_test0 (a:BN.t) : W64.t = {
+    var aux_0: bool;
+    var aux: W64.t;
+    
+    var res_0:W64.t;
+    var is_zero:W64.t;
+    var zf:bool;
+    
+    leakages <- LeakAddr([]) :: leakages;
+    aux <- (W64.of_int 0);
+    res_0 <- aux;
+    leakages <- LeakAddr([]) :: leakages;
+    aux <- (W64.of_int 1);
+    is_zero <- aux;
+    leakages <- LeakAddr([]) :: leakages;
+    aux_0 <@ __bn_test0_zf (a);
+    zf <- aux_0;
+    leakages <- LeakAddr([]) :: leakages;
+    aux <- (zf ? is_zero : res_0);
+    res_0 <- aux;
+    return (res_0);
+  }
+  
+  proc _bn_test0 (a:BN.t) : W64.t = {
+    var aux: W64.t;
+    
+    var r:W64.t;
+    
+    leakages <- LeakAddr([]) :: leakages;
+    aux <@ __bn_test0 (a);
+    r <- aux;
+    return (r);
+  }
+  
+  proc __bn_copy (a:BN.t) : BN.t = {
+    var aux: int;
+    var aux_0: W64.t;
+    
+    var r:BN.t;
+    var i:int;
+    var t:W64.t;
+    r <- witness;
+    leakages <- LeakFor(0,nlimbs) :: LeakAddr([]) :: leakages;
+    i <- 0;
+    while (i < nlimbs) {
+      leakages <- LeakAddr([i]) :: leakages;
+      aux_0 <- a.[i];
+      t <- aux_0;
+      leakages <- LeakAddr([]) :: leakages;
+      aux_0 <- t;
+      leakages <- LeakAddr([i]) :: leakages;
+      r.[i] <- aux_0;
+      i <- i + 1;
+    }
+    return (r);
+  }
+  
+  proc __bn_copy2 (a:BN.t, r:BN.t) : BN.t = {
+    var aux: int;
+    var aux_0: W64.t;
+    
+    var i:int;
+    var t:W64.t;
+    
+    leakages <- LeakFor(0,nlimbs) :: LeakAddr([]) :: leakages;
+    i <- 0;
+    while (i < nlimbs) {
+      leakages <- LeakAddr([i]) :: leakages;
+      aux_0 <- a.[i];
+      t <- aux_0;
+      leakages <- LeakAddr([]) :: leakages;
+      aux_0 <- t;
+      leakages <- LeakAddr([i]) :: leakages;
+      r.[i] <- aux_0;
+      i <- i + 1;
+    }
+    return (r);
+  }
+  
+  proc __bn_cmov (cond:bool, a:BN.t, b:BN.t) : 
+  BN.t = {
+    var aux: int;
+    var aux_0: W64.t;
+    
+    var i:int;
+    var t:W64.t;
+    
+    leakages <- LeakFor(0,nlimbs) :: LeakAddr([]) :: leakages;
+    i <- 0;
+    while (i < nlimbs) {
+      leakages <- LeakAddr([i]) :: leakages;
+      aux_0 <- a.[i];
+      t <- aux_0;
+      leakages <- LeakAddr([i]) :: leakages;
+      aux_0 <- (cond ? b.[i] : t);
+      t <- aux_0;
+      leakages <- LeakAddr([]) :: leakages;
+      aux_0 <- t;
+      leakages <- LeakAddr([i]) :: leakages;
+      a.[i] <- aux_0;
+      i <- i + 1;
+    }
+    return (a);
+  }
+  
+  proc __bn_set0 (a:BN.t) : BN.t = {
+    var aux_0: int;
+    var aux: W64.t;
+    
+    var t:W64.t;
+    var i:int;
+    
+    leakages <- LeakAddr([]) :: leakages;
+    aux <- (W64.of_int 0);
+    t <- aux;
+    leakages <- LeakFor(0,nlimbs) :: LeakAddr([]) :: leakages;
+    i <- 0;
+    while (i < nlimbs) {
+      leakages <- LeakAddr([]) :: leakages;
+      aux <- t;
+      leakages <- LeakAddr([i]) :: leakages;
+      a.[i] <- aux;
+      i <- i + 1;
+    }
+    return (a);
+  }
+  
+  proc __bn_add1c (a:BN.t, b:W64.t) : bool * BN.t = {
+    var aux: bool;
+    var aux_1: int;
+    var aux_0: W64.t;
+    
+    var cf:bool;
+    var i:int;
+    
+    leakages <- LeakAddr([0]) :: leakages;
+    (aux, aux_0) <- adc_64 a.[0] b false;
+    cf <- aux;
+    leakages <- LeakAddr([0]) :: leakages;
+    a.[0] <- aux_0;
+    leakages <- LeakFor(1,nlimbs) :: LeakAddr([]) :: leakages;
+    i <- 1;
+    while (i < nlimbs) {
+      leakages <- LeakAddr([i]) :: leakages;
+      (aux, aux_0) <- adc_64 a.[i] (W64.of_int 0) cf;
+      cf <- aux;
+      leakages <- LeakAddr([i]) :: leakages;
+      a.[i] <- aux_0;
+      i <- i + 1;
+    }
+    return (cf, a);
+  }
+  
+  proc __bn_addc (a:BN.t, b:BN.t) : bool *
+                                                          BN.t = {
+    var aux_0: bool;
+    var aux_1: int;
+    var aux: W64.t;
+    
+    var cf:bool;
+    var t:W64.t;
+    var i:int;
+    
+    leakages <- LeakAddr([0]) :: leakages;
+    aux <- b.[0];
+    t <- aux;
+    leakages <- LeakAddr([0]) :: leakages;
+    (aux_0, aux) <- adc_64 a.[0] t false;
+    cf <- aux_0;
+    leakages <- LeakAddr([0]) :: leakages;
+    a.[0] <- aux;
+    leakages <- LeakFor(1,nlimbs) :: LeakAddr([]) :: leakages;
+    i <- 1;
+    while (i < nlimbs) {
+      leakages <- LeakAddr([i]) :: leakages;
+      aux <- b.[i];
+      t <- aux;
+      leakages <- LeakAddr([i]) :: leakages;
+      (aux_0, aux) <- adc_64 a.[i] t cf;
+      cf <- aux_0;
+      leakages <- LeakAddr([i]) :: leakages;
+      a.[i] <- aux;
+      i <- i + 1;
+    }
+    return (cf, a);
+  }
+  
+  proc _bn_addc (a:BN.t, b:BN.t) : bool *
+                                                         BN.t = {
+    var aux: bool;
+    var aux_0: BN.t;
+    
+    var cf:bool;
+    
+    leakages <- LeakAddr([]) :: leakages;
+    (aux, aux_0) <@ __bn_addc (a, b);
+    cf <- aux;
+    a <- aux_0;
+    return (cf, a);
+  }
+  
+  proc __bn_subc (a:BN.t, b:BN.t) : bool *
+                                                          BN.t = {
+    var aux_0: bool;
+    var aux_1: int;
+    var aux: W64.t;
+    
+    var cf:bool;
+    var t:W64.t;
+    var i:int;
+    
+    leakages <- LeakAddr([0]) :: leakages;
+    aux <- b.[0];
+    t <- aux;
+    leakages <- LeakAddr([0]) :: leakages;
+    (aux_0, aux) <- sbb_64 a.[0] t false;
+    cf <- aux_0;
+    leakages <- LeakAddr([0]) :: leakages;
+    a.[0] <- aux;
+    leakages <- LeakFor(1,nlimbs) :: LeakAddr([]) :: leakages;
+    i <- 1;
+    while (i < nlimbs) {
+      leakages <- LeakAddr([i]) :: leakages;
+      aux <- b.[i];
+      t <- aux;
+      leakages <- LeakAddr([i]) :: leakages;
+      (aux_0, aux) <- sbb_64 a.[i] t cf;
+      cf <- aux_0;
+      leakages <- LeakAddr([i]) :: leakages;
+      a.[i] <- aux;
+      i <- i + 1;
+    }
+    return (cf, a);
+  }
+  
+  proc __bn_lt_cf (a:BN.t, b:BN.t) : bool = {
+    var aux_0: bool;
+    var aux_1: int;
+    var aux: W64.t;
+    
+    var cf:bool;
+    var t:W64.t;
+    var i:int;
+    
+    leakages <- LeakAddr([0]) :: leakages;
+    aux <- a.[0];
+    t <- aux;
+    leakages <- LeakAddr([0]) :: leakages;
+    (aux_0, aux) <- sbb_64 t b.[0] false;
+    cf <- aux_0;
+    t <- aux;
+    leakages <- LeakFor(1,nlimbs) :: LeakAddr([]) :: leakages;
+    i <- 1;
+    while (i < nlimbs) {
+      leakages <- LeakAddr([i]) :: leakages;
+      aux <- a.[i];
+      t <- aux;
+      leakages <- LeakAddr([i]) :: leakages;
+      (aux_0, aux) <- sbb_64 t b.[i] cf;
+      cf <- aux_0;
+      t <- aux;
+      i <- i + 1;
+    }
+    return (cf);
+  }
+  
+  proc _bn_subc (a:BN.t, b:BN.t) : bool *
+                                                         BN.t = {
+    var aux: bool;
+    var aux_0: BN.t;
+    
+    var cf:bool;
+    
+    leakages <- LeakAddr([]) :: leakages;
+    (aux, aux_0) <@ __bn_subc (a, b);
+    cf <- aux;
+    a <- aux_0;
+    return (cf, a);
+  }
+  
+  proc __bn_rnd (a:BN.t) : BN.t = {
+    leakages <- LeakAddr([]) :: leakages;
+    a <$ BN.bn_rnd;
+    return a;
+  }
+  
+  proc __bn_rsample (a:BN.t, bnd:BN.t) : BN.t = {
+    var aux_0: bool;
+    var aux: BN.t;
+    
+    var cf:bool;
+    
+    leakages <- LeakAddr([]) :: leakages;
+    aux <@ __bn_rnd (a);
+    a <- aux;
+    leakages <- LeakAddr([]) :: leakages;
+    aux_0 <@ __bn_lt_cf (a, bnd);
+    cf <- aux_0;
+    leakages <- LeakCond((! cf)) :: LeakAddr([]) :: leakages;
+    
+    while ((! cf)) {
+      leakages <- LeakAddr([]) :: leakages;
+      aux <@ __bn_rnd (a);
+      a <- aux;
+      leakages <- LeakAddr([]) :: leakages;
+      aux_0 <@ __bn_lt_cf (a, bnd);
+      cf <- aux_0;
+    leakages <- LeakCond((! cf)) :: LeakAddr([]) :: leakages;
+    
+    }
+    return (a);
+  }
+}.
+
+(** M vs. Mleak *)
+equiv __bn_load_proj:
+ M.__bn_load ~ Mleak.__bn_load : ={arg, Glob.mem} ==> ={res}
+ by sim.
+
+equiv __bn_store_proj:
+ M.__bn_store ~ Mleak.__bn_store : ={arg, Glob.mem} ==> ={res, Glob.mem}
+ by sim.
+
+equiv __bn_eq_zf_proj:
+ M.__bn_eq_zf ~ Mleak.__bn_eq_zf : ={arg} ==> ={res}
+ by sim.
+
+equiv __bn_eq_proj:
+ M.__bn_eq ~ Mleak.__bn_eq : ={arg} ==> ={res}
+ by sim.
+
+equiv _bn_eq_proj:
+ M._bn_eq ~ Mleak._bn_eq : ={arg} ==> ={res}
+ by sim.
+
+equiv _bn_eq__proj:
+ M._bn_eq_ ~ Mleak._bn_eq_ : ={arg} ==> ={res}
+ by sim.
+
+equiv __bn_test0_zf_proj:
+ M.__bn_test0_zf ~ Mleak.__bn_test0_zf : ={arg} ==> ={res}
+ by sim.
+
+equiv __bn_test0_proj:
+ M.__bn_test0 ~ Mleak.__bn_test0 : ={arg} ==> ={res}
+ by sim.
+
+equiv _bn_test0_proj:
+ M._bn_test0 ~ Mleak._bn_test0 : ={arg} ==> ={res}
+ by sim.
+
+equiv __bn_copy_proj:
+ M.__bn_copy ~ Mleak.__bn_copy : ={arg} ==> ={res}
+ by sim.
+
+equiv __bn_copy2_proj:
+ M.__bn_copy2 ~ Mleak.__bn_copy2 : ={arg} ==> ={res}
+ by sim.
+
+equiv __bn_cmov_proj:
+ M.__bn_cmov ~ Mleak.__bn_cmov : ={arg} ==> ={res}
+ by sim.
+
+equiv __bn_set0_proj:
+ M.__bn_set0 ~ Mleak.__bn_set0 : ={arg} ==> ={res}
+ by sim.
+
+equiv __bn_add1c_proj:
+ M.__bn_add1c ~ Mleak.__bn_add1c : ={arg} ==> ={res}
+ by sim.
+
+equiv __bn_addc_proj:
+ M.__bn_addc ~ Mleak.__bn_addc : ={arg} ==> ={res}
+ by sim.
+
+equiv _bn_addc_proj:
+ M._bn_addc ~ Mleak._bn_addc : ={arg} ==> ={res}
+ by sim.
+
+equiv __bn_subc_proj:
+ M.__bn_subc ~ Mleak.__bn_subc : ={arg} ==> ={res}
+ by sim.
+
+equiv _bn_subc_proj:
+ M._bn_subc ~ Mleak._bn_subc : ={arg} ==> ={res}
+ by sim.
+
+equiv __bn_lt_cf_proj:
+ M.__bn_lt_cf ~ Mleak.__bn_lt_cf : ={arg} ==> ={res}
+ by sim.
+
+equiv __bn_rnd_proj:
+ M.__bn_rnd ~ Mleak.__bn_rnd : ={arg} ==> ={res}
+ by sim.
+
+equiv __bn_rsample_proj:
+ M.__bn_rsample ~ Mleak.__bn_rsample : ={arg} ==> ={res}
+ by sim.
+
+
+(* ct property *)
+
+equiv __bn_load_ct:
+ Mleak.__bn_load ~ Mleak.__bn_load : 
+  ={a, Mleak.leakages} ==> ={Mleak.leakages}.
+proof. by proc; sim. qed.
+
+equiv __bn_store_ct:
+ Mleak.__bn_store ~ Mleak.__bn_store : 
+  ={a, Mleak.leakages} ==> ={Mleak.leakages}.
+proof. by proc; sim. qed.
+
+equiv __bn_eq_zf_ct:
+ Mleak.__bn_eq_zf ~ Mleak.__bn_eq_zf : 
+  ={Mleak.leakages} ==> ={Mleak.leakages}.
+proof. by proc; sim. qed.
+
+equiv __bn_eq_ct:
+ Mleak.__bn_eq ~ Mleak.__bn_eq :
+  ={Mleak.leakages} ==> ={Mleak.leakages}.
+proof.
+proc; wp.
+by call __bn_eq_zf_ct; auto => />.
+qed.
+
+equiv _bn_eq_ct:
+ Mleak._bn_eq ~ Mleak._bn_eq :
+  ={Mleak.leakages} ==> ={Mleak.leakages}.
+proof. 
+proc; wp.
+by call __bn_eq_ct; auto => />.
+qed.
+
+equiv _bn_eq__ct:
+ Mleak._bn_eq_ ~ Mleak._bn_eq_ :
+  ={Mleak.leakages} ==> ={Mleak.leakages}.
+proof. 
+proc; wp.
+by call _bn_eq_ct; auto => />.
+qed.
+
+equiv __bn_test0_zf_ct:
+ Mleak.__bn_test0_zf ~ Mleak.__bn_test0_zf :
+  ={Mleak.leakages} ==> ={Mleak.leakages}.
+proof. by proc; sim. qed.
+
+equiv __bn_test0_ct:
+ Mleak.__bn_test0 ~ Mleak.__bn_test0 :
+  ={Mleak.leakages} ==> ={Mleak.leakages}.
+proof.
+proc; wp.
+by call __bn_test0_zf_ct; auto => />.
+qed.
+
+equiv _bn_test0_ct:
+ Mleak._bn_test0 ~ Mleak._bn_test0 :
+  ={Mleak.leakages} ==> ={Mleak.leakages}.
+proof.
+proc; wp.
+by call __bn_test0_ct; auto => />.
+qed.
+
+equiv __bn_copy_ct:
+ Mleak.__bn_copy ~ Mleak.__bn_copy :
+  ={Mleak.leakages} ==> ={Mleak.leakages}.
+proof. by proc; sim. qed.
+
+equiv __bn_copy2_ct:
+ Mleak.__bn_copy2 ~ Mleak.__bn_copy2 :
+  ={Mleak.leakages} ==> ={Mleak.leakages}.
+proof. by proc; sim. qed.
+
+equiv __bn_cmov_ct:
+ Mleak.__bn_cmov ~ Mleak.__bn_cmov :
+  ={Mleak.leakages} ==> ={Mleak.leakages}.
+proof. by proc; sim. qed.
+
+equiv __bn_set0_ct:
+ Mleak.__bn_set0 ~ Mleak.__bn_set0 :
+  ={Mleak.leakages} ==> ={Mleak.leakages}.
+proof. by proc; sim. qed.
+
+equiv __bn_add1c_ct:
+ Mleak.__bn_add1c ~ Mleak.__bn_add1c :
+  ={Mleak.leakages} ==> ={Mleak.leakages}.
+proof. by proc; sim. qed.
+
+equiv __bn_addc_ct:
+ Mleak.__bn_addc ~ Mleak.__bn_addc :
+  ={Mleak.leakages} ==> ={Mleak.leakages}.
+proof. by proc; sim. qed.
+
+equiv _bn_addc_ct:
+ Mleak._bn_addc ~ Mleak._bn_addc :
+  ={Mleak.leakages} ==> ={Mleak.leakages}.
+proof.
+proc; wp.
+by call __bn_addc_ct; auto => />.
+qed.
+
+equiv __bn_subc_ct:
+ Mleak.__bn_subc ~ Mleak.__bn_subc :
+  ={Mleak.leakages} ==> ={Mleak.leakages}.
+proof. by proc; sim. qed.
+
+equiv _bn_subc_ct:
+ Mleak._bn_subc ~ Mleak._bn_subc :
+  ={Mleak.leakages} ==> ={Mleak.leakages}.
+proof.
+proc; wp.
+by call __bn_subc_ct; auto => />.
+qed.
+
+equiv __bn_lt_cf_ct:
+ Mleak.__bn_lt_cf ~ Mleak.__bn_lt_cf :
+  ={Mleak.leakages} ==> ={Mleak.leakages}.
+proof. by proc; sim. qed.
+
+equiv __bn_rnd_ct:
+ Mleak.__bn_rnd ~ Mleak.__bn_rnd :
+  ={Mleak.leakages} ==> ={Mleak.leakages}.
+proof. by proc; sim. qed.
+
+equiv __bn_rsample_ct:
+ Mleak.__bn_rsample ~ Mleak.__bn_rsample :
+  ={bnd, Mleak.leakages} ==> ={Mleak.leakages}.
+proof.
+proc; wp.
+while (={bnd, cf, Mleak.leakages}).
+ wp; call (: ={arg,Mleak.leakages} ==> ={res, Mleak.leakages}); first by sim.
+ by inline*; auto => /> *.
+wp; call (: ={arg,Mleak.leakages} ==> ={res, Mleak.leakages}); first by sim.
+by inline*; auto => /> *.
+qed.
+
+
+(**
+  * Leakage-freeness for probabilistic programs
+  * ===========================================
+  *
+  * The following development illustrates the
+  * proof of Leakage-freeness for the rejection
+  * sampling procedure [__bn_rsample]. It relies
+  * on the definitions and lemmas formalised in
+  * [PRHL_Defs], presented on paper ...
+***)
+require import PRHL_Defs.
+
+(** The following theories instantiate the
+ abstract developments for individual procedures.*)
+theory CT_bn_lt.
+clone import CT_Meta as Meta
+ with type pin_t <- unit, (*  *)
+      type sin_t <- BN.t*BN.t, (* a, b *)
+      type out_t <- bool. (* res *)
+
+module JI = {
+ proc main(pin: unit, sin: BN.t*BN.t) : bool = {
+  var r;
+  r <@ M.__bn_lt_cf(sin.`1,sin.`2);
+  return r;
+ }
+}.
+
+lemma stateless_JI &m x: (glob JI){m} = x
+ by done.
+
+module JR = {
+ proc main(pin: unit, sin: BN.t*BN.t) : bool = {
+  var r;
+  r <@ Mleak.__bn_lt_cf(sin.`1,sin.`2);
+  return r;
+ }
+ proc mainG(pin: unit, sin: BN.t*BN.t) : bool * leakages_t = {
+  var r;
+  r <@ Mleak.__bn_lt_cf(sin.`1,sin.`2);
+  return (r, Mleak.leakages);
+ }
+}.
+
+lemma proj_JR_JI:
+ equiv [ JR.main ~ JI.main
+       : ={pin, sin} ==> ={res} ]
+ by sim.
+
+lemma globJR:
+ equiv [ JR.main ~ JR.mainG
+       : ={pin,sin,glob JR}
+         ==> ={glob JR} /\ res{2} = (res{1},glob JR){2} ].
+proof.
+proc*; inline JR.main JR.mainG.
+wp; call (: ={arg,glob JR} ==> ={res,glob JR}) => //.
+ by proc; sim.
+by auto.
+qed.
+
+lemma prMuE P pin sin &m:
+ Pr[ JR.main(pin,sin) @ &m : P (res,glob JR)]
+ = RealSeries.sum (fun (x:_*_) => Pr [JR.main(pin,sin) @ &m : P (res,glob JR) /\ res=x.`1 /\ (glob JR)=x.`2]).
+proof.
+have ->: Pr[JR.main(pin, sin) @ &m : P (res,glob JR)]
+  = Pr[JR.mainG(pin, sin) @ &m : P res].
+ byequiv => //.
+ by conseq globJR => /> // /#.
+rewrite Pr [muE].
+apply RealSeries.eq_sum; move => [r l].
+rewrite eq_sym.
+by byequiv globJR => /> /#.
+qed.
+
+end CT_bn_lt.
+
+lemma CT_bn_lt:
+ equiv[ CT_bn_lt.Meta.RSim(CT_bn_lt.JI, CT_bn_lt.JR).main ~ CT_bn_lt.Meta.SimR(CT_bn_lt.JI, CT_bn_lt.JR).main :
+  ={pin, sin, glob CT_bn_lt.JR} ==> ={res, glob CT_bn_lt.JR}].
+proof.
+apply (CT_bn_lt.Meta.ct_det_CT CT_bn_lt.JR CT_bn_lt.JI).
++ by apply CT_bn_lt.stateless_JI.
++ by apply CT_bn_lt.proj_JR_JI.
++ by apply CT_bn_lt.prMuE.
++ by proc; call __bn_lt_cf_ct; auto => />.
+exists (fun _ (x:_*_) => bn x.`1 < bn x.`2) => ? [a b].
+by proc; ecall (__bn_lt_cf_h a b); auto.
+qed.
+
+lemma CT'_bn_lt:
+ equiv[ CT_bn_lt.JR.main ~ CT_bn_lt.Meta.SimR(CT_bn_lt.JI, CT_bn_lt.JR).main :
+  ={pin, sin, glob CT_bn_lt.JR} ==> ={res, glob CT_bn_lt.JR}].
+proof.
+apply (CT_bn_lt.Meta.ll_CT CT_bn_lt.JR CT_bn_lt.JI _ _ _ _ CT_bn_lt).
++ by apply CT_bn_lt.stateless_JI.
++ by apply CT_bn_lt.proj_JR_JI.
++ by apply CT_bn_lt.prMuE.
+by proc; call __bn_lt_cf_ll.
+qed.
+
+
+theory CT_bn_rnd.
+
+clone import CT_Meta as Meta
+ with type pin_t <- unit, (*  *)
+      type sin_t <- BN.t, (* a *)
+      type out_t <- BN.t. (* res *)
+
+module JI = {
+ proc main(pin: unit, sin: BN.t) : BN.t = {
+  var r;
+  r <@ M.__bn_rnd(sin);
+  return r;
+ }
+}.
+
+lemma stateless_JI &m x: (glob JI){m} = x
+ by done.
+
+module JR = {
+ proc main(pin: unit, sin: BN.t) : BN.t = {
+  var r;
+  r <@ Mleak.__bn_rnd(sin);
+  return r;
+ }
+ proc mainG(pin: unit, sin: BN.t) : BN.t * leakages_t = {
+  var r;
+  r <@ Mleak.__bn_rnd(sin);
+  return (r, Mleak.leakages);
+ }
+}.
+
+lemma proj_JR_JI:
+ equiv [ JR.main ~ JI.main
+       : ={pin, sin} ==> ={res} ]
+ by sim.
+
+lemma globJR:
+ equiv [ JR.main ~ JR.mainG
+       : ={pin,sin,glob JR}
+         ==> ={glob JR} /\ res{2} = (res{1},glob JR){2} ].
+proof.
+proc*; inline JR.main JR.mainG.
+wp; call (: ={arg,glob JR} ==> ={res,glob JR}) => //.
+ by proc; sim.
+by auto.
+qed.
+
+lemma prMuE P pin sin &m:
+ Pr[ JR.main(pin,sin) @ &m : P (res,glob JR)]
+ = RealSeries.sum (fun (x:_*_) => Pr [JR.main(pin,sin) @ &m : P (res,glob JR) /\ res=x.`1 /\ (glob JR)=x.`2]).
+proof.
+have ->: Pr[JR.main(pin, sin) @ &m : P (res,glob JR)]
+  = Pr[JR.mainG(pin, sin) @ &m : P res].
+ byequiv => //.
+ by conseq globJR => /> // /#.
+rewrite Pr [muE].
+apply RealSeries.eq_sum; move => [r l].
+rewrite eq_sym.
+by byequiv globJR => /> /#.
+qed.
+
+end CT_bn_rnd.
+
+lemma CT_bn_rnd:
+ equiv[ CT_bn_rnd.Meta.RSim(CT_bn_rnd.JI, CT_bn_rnd.JR).main ~ CT_bn_rnd.Meta.SimR(CT_bn_rnd.JI, CT_bn_rnd.JR).main :
+  ={pin, sin, glob CT_bn_rnd.JR} ==> ={res, glob CT_bn_rnd.JR}].
+proof. by proc; inline*; auto. qed.
+
+lemma CT'_bn_rnd:
+ equiv[ CT_bn_rnd.JR.main ~ CT_bn_rnd.Meta.SimR(CT_bn_rnd.JI, CT_bn_rnd.JR).main :
+  ={pin, sin, glob CT_bn_rnd.JR} ==> ={res, glob CT_bn_rnd.JR}].
+proof.
+apply (CT_bn_rnd.Meta.ll_CT CT_bn_rnd.JR CT_bn_rnd.JI _ _ _ _ CT_bn_rnd).
++ by apply CT_bn_rnd.stateless_JI.
++ by apply CT_bn_rnd.proj_JR_JI.
++ by apply CT_bn_rnd.prMuE.
+by proc; islossless; smt(bn_rnd_ll).
+qed.
+
+
+
+
+theory CT_bn_rsample.
+
+clone import CT_Meta as Meta
+ with type pin_t <- BN.t, (* bnd *)
+      type sin_t <- BN.t, (* a *)
+      type out_t <- BN.t. (* res *)
+
+module JI = {
+ proc main(pin : BN.t, sin: BN.t) : BN.t = {
+  var r;
+  r <@ M.__bn_rsample(sin,pin);
+  return r;
+ }
+}.
+
+lemma stateless_JI &m x: (glob JI){m} = x
+ by done.
+
+module JR = {
+ proc main(pin : BN.t, sin: BN.t) : BN.t = {
+  var r;
+  r <@ Mleak.__bn_rsample(sin,pin);
+  return r;
+ }
+ proc mainG(pin : BN.t, sin: BN.t) : BN.t * leakages_t = {
+  var r;
+  r <@ Mleak.__bn_rsample(sin,pin);
+  return (r, Mleak.leakages);
+ }
+}.
+
+lemma proj_JR_JI:
+ equiv [ JR.main ~ JI.main
+       : ={pin, sin} ==> ={res} ]
+ by sim.
+
+lemma globJR:
+ equiv [ JR.main ~ JR.mainG
+       : ={pin,sin,glob JR}
+         ==> ={glob JR} /\ res{2} = (res{1},glob JR){2} ].
+proof.
+proc*; inline JR.main JR.mainG.
+wp; call (: ={arg,glob JR} ==> ={res,glob JR}) => //.
+ by proc; sim.
+by auto.
+qed.
+
+lemma prMuE P pin sin &m:
+ Pr[ JR.main(pin,sin) @ &m : P (res,glob JR)]
+ = RealSeries.sum (fun (x:_*_) => Pr [JR.main(pin,sin) @ &m : P (res,glob JR) /\ res=x.`1 /\ (glob JR)=x.`2]).
+proof.
+have ->: Pr[JR.main(pin, sin) @ &m : P (res,glob JR)]
+  = Pr[JR.mainG(pin, sin) @ &m : P res].
+ byequiv => //.
+ by conseq globJR => /> // /#.
+rewrite Pr [muE].
+apply RealSeries.eq_sum; move => [r l].
+rewrite eq_sym.
+by byequiv globJR => /> /#.
+qed.
+
+end CT_bn_rsample.
+
+
+(**
+  * PROOF OF LEAKAGE-FREENESS FOR __bn_rsample
+***)
+
+(* Auxiliary theory for decoupling the sampling from leaked events *)
+abstract theory SampleEventSwap.
+
+type in_t.
+type out_t.
+
+require import DBool DProd.
+import Biased.
+
+module SampleEvent = {
+ proc sample(i: in_t, d: in_t -> out_t distr, P: in_t -> out_t -> bool): out_t * bool = {
+  var b, x;
+  x <$ d i;
+  b <- P i x;
+  return (x, b);
+ }
+ proc sampleEv(i: in_t, d: in_t -> out_t distr, P: in_t -> out_t -> bool): out_t * bool = {
+  var b, x;
+  b <$ dbiased (mu (d i) (P i));
+  x <$ if b then dcond (d i) (P i) else dcond (d i) (predC (P i));
+  return (x, b);
+ }
+}.
+
+
+clone DLetSampling as LS with
+ type t <- bool,
+ type u <- out_t.
+
+equiv sample_sampleEv:
+ SampleEvent.sample ~ SampleEvent.sampleEv:
+ ={i, d, P} /\ is_lossless (d i){2} 
+ ==> ={res}.
+proof.
+proc; simplify; wp.
+case: ((mu (d i) (P i)){2}=0%r).
+ seq 0 1: (#pre /\ !b{2}).
+  rnd{2}; auto => /> &m Hll Hb; split; first by apply dbiased_ll.
+  by move=> _ b; rewrite Hb dbiased0 supp_dunit.
+ rnd; auto => /> &m Hll Hb0 Hb; split.
+  move=> xR; rewrite dcond_supp; move=> [Hx1 Hx2].
+  by rewrite dcond1E Hx2 /= mu_not Hll Hb0 /=.
+ move => H xL Hx; split.
+  by rewrite dcond_supp Hx /predC /=; apply (eq0_mu (d{m} i{m}) (P{m} i{m})).
+ by rewrite dcond_supp Hx /predC /= /#.
+case: ((mu (d i) (P i)){2}=1%r).
+ seq 0 1: (#pre /\ b{2}).
+  rnd{2}; auto => /> &m Hll _ Hb; split; first by apply dbiased_ll.
+  by move=> _ b; rewrite Hb dbiased1 supp_dunit.
+ rnd; auto => /> &m Hll _ Hb1 Hb; split.
+  move=> xR; rewrite dcond_supp; move=> [Hx1 Hx2].
+  by rewrite dcond1E Hx2 Hb1.
+ move => _ xL Hx; split.
+  rewrite dcond_supp Hx /=. 
+  apply (mu_in_weight (P{m} i{m}) (d{m} i{m})) => //.
+  by rewrite Hb1 Hll.
+ by rewrite dcond_supp Hx /#.
+transitivity{1} { x <@ LS.SampleDLet.sample(dbiased (mu (d i) (P i)), fun b=> if b then dcond (d i) (P i) else dcond (d i) (predC (P i))); }
+ (={i,d,P} /\ is_lossless (d i){2} /\ 0%r < (mu (d i) (P i)){2} < 1%r
+  ==> ={x,i,d,P} /\ is_lossless (d i){2} /\ 0%r < (mu (d i) (P i)){2} < 1%r)
+ (={i,d,P} /\ is_lossless (d i){2} /\ 0%r < (mu (d i) (P i)){2} < 1%r ==> ={x} /\ P{1} i{1} x{1}=b{2}) => //.
+  by move=> /> &m Hll Hbias1 Hbias2; exists P{m} d{m} i{m}; smt(mu_bounded).
+ inline*; auto => /> &m Hll Hbias1 Hbias2; split.
+  move=> xR.
+  by rewrite -marginal_sampling_pred //.
+ move => H xL HxL.
+ rewrite supp_dlet.
+ case: (P{m} i{m} xL) => bL.
+  exists true => /=.
+  rewrite supp_dbiased 1:/#.
+  by rewrite dcond_supp.
+ exists false => /=.
+ rewrite supp_dbiased 1:/#.
+ by rewrite dcond_supp.
+transitivity{1} { x <@ LS.SampleDep.sample(dbiased (mu (d i) (P i)), fun b=> if b then dcond (d i) (P i) else dcond (d i) (predC (P i))); }
+ (={i,d,P} /\ 0%r < (mu (d i) (P i)){2} < 1%r ==> ={x,i,d,P} /\ 0%r < (mu (d i) (P i)){2} < 1%r)
+ (={i,d,P} /\ 0%r < (mu (d i) (P i)){2} < 1%r ==> ={x} /\ P{1} i{1} x{1}=b{2}) => //.
+  by move=> /> &m Hll Hbias1 Hbias2; exists P{m} d{m} i{m}; auto.
+ by symmetry; call LS.SampleDepDLet => //=.
+inline*; auto => /> &m Hbias1 Hbias2 b Hb xL.
+by case: (b) => Cb; rewrite dcond_supp /#.
+qed.
+
+end SampleEventSwap.
+
+
+
+(** Auxiliary theory to perform the eager/lazy sampling on the rejection loop *)
+abstract theory RejectionLoop.
+
+type t.
+
+op dt: t distr.
+op p : t -> t -> bool.
+(* workaround to get a lossless distribution on the underlying RO (required in EC's
+ PROM.ec library *)
+op t0: t.
+op p_ll bnd x = bnd=t0 \/ p bnd x.
+
+axiom dt_ll: is_lossless dt.
+axiom t0_ll: 0%r < mu1 dt t0.
+axiom p_t0E: p t0=pred0.
+axiom p_t0P bnd: bnd <> t0 => p bnd t0.
+axiom dtPN_ll bnd: 0%r < mu dt (predC (p bnd)).
+
+lemma dcondP_ll bnd b:
+ is_lossless (if b then dcond dt (p_ll bnd) else dcond dt (predC (p bnd))).
+proof.
+case: (b) => ?.
+ rewrite /p_ll dcond_ll.
+ case: (bnd=t0) => E /=; first smt(dt_ll).
+ apply (StdOrder.RealOrder.ltr_le_trans (mu1 dt t0) _ _ t0_ll).
+ apply mu_le => x _ @/pred1 /= ->.
+ by apply p_t0P.
+rewrite dcond_ll; exact dtPN_ll.
+qed.
+
+lemma p_llE bnd:
+ bnd <> t0 => p_ll bnd = p bnd by smt().
+
+module type AdvLoop = {
+  proc loop_init(b: bool): unit
+  proc loop_body(b: bool): unit
+}.
+
+require import DBool.
+import Biased.
+
+module RejLoop(L:AdvLoop) = {
+  proc loopEager (bnd: t) = {
+    var x, b;
+    b <$ dbiased (mu dt (p bnd));
+    x <$ if b then dcond dt (p bnd)
+              else dcond dt (predC (p bnd));
+    L.loop_init(b);
+    while (! b) {
+      b <$ dbiased (mu dt (p bnd));
+      x <$ if b then dcond dt (p bnd)
+                else dcond dt (predC (p bnd));
+      L.loop_body(b);
+    }
+    return x;
+  }
+  proc loopLazy (bnd: t) = {
+    var x, b;
+    b <$ dbiased (mu dt (p bnd));
+    L.loop_init(b);
+    while (!b) {
+      b <$ dbiased (mu dt (p bnd));
+      L.loop_body(b);
+    }
+    x <$ dcond dt (p bnd);
+    return x;
+  }
+}.
+
+
+require import PROM SmtMap.
+
+clone import PROM.FullRO as ROx with
+    type in_t    <- t*bool,
+    type out_t   <- t, 
+    type d_in_t  <- t,
+    type d_out_t <- t,
+    op   dout    <- fun y:_*_=> if y.`2
+                            then dcond dt (p_ll y.`1)
+                            else dcond dt (predC (p y.`1))
+  proof *.
+
+module RejLoop_D (L:AdvLoop) (O: RO) = {
+ proc distinguish(bnd): t = {
+  var b, x;
+  b <$ dbiased (mu dt (p bnd));
+  O.sample((bnd,b));
+  L.loop_init(b);
+  while (!b) {
+    O.rem((bnd,b));
+    b <$ dbiased (mu dt (p bnd));
+    O.sample((bnd,b));
+    L.loop_body(b);
+  }
+  x <@ O.get((bnd,b));
+  return x;
+ }
+}.
+
+section.
+
+declare module L <: AdvLoop {+Mleak}.
+
+module RejLoopD = RejLoop_D(L).
+
+lemma pr_loopEager_t0 &m:
+ Pr[RejLoop(L).loopEager(t0) @ &m : true] = 0%r.
+proof.
+byphoare (:arg=t0 ==> _) => //.
+proc; hoare.
+while (!b /\ bnd=t0) => //.
+ call (:true).
+ auto => /> &1 b b'.
+ by rewrite p_t0E mu0 dbiased0 supp_dunit => -> /=.
+call (:true); auto => /> b.
+by rewrite p_t0E mu0 dbiased0 supp_dunit => -> /=.
+qed.
+
+lemma pr_loopLazy_t0 &m:
+ Pr[RejLoop(L).loopLazy(t0) @ &m : true] = 0%r.
+proof.
+byphoare (:arg=t0 ==> _) => //.
+proc; hoare.
+seq 3: (bnd=t0).
+ while (!b /\ bnd=t0) => //.
+  call (:true).
+  auto => /> &1 b b'.
+  by rewrite p_t0E mu0 dbiased0 supp_dunit => -> /=.
+ call (:true); auto => /> b.
+ by rewrite p_t0E mu0 dbiased0 supp_dunit => -> /=.
+by auto => /> x; rewrite p_t0E dcond_supp /pred0 /=.
+qed.
+
+equiv rejloop_t0_eq:
+ RejLoop(L).loopEager ~ RejLoop(L).loopLazy
+ : ={bnd} /\ bnd{2}=t0 ==> ={res, glob L}.
+proof.
+bypr (res,glob L){1} (res,glob L){2} => //.
+move=> /> &1 &2 [r l] -> ->.
+have ->: Pr[RejLoop(L).loopEager(t0) @ &1 : (res, (glob L)) = (r, l)] = 0%r.
+ by rewrite -(pr_loopEager_t0 &1); smt(mu_le pr_loopEager_t0).
+by rewrite eq_sym -(pr_loopLazy_t0 &1); smt(mu_le pr_loopLazy_t0).
+qed.
+
+equiv rejloop_eq:
+ RejLoop(L).loopEager ~ RejLoop(L).loopLazy
+ : ={bnd, glob L} ==> ={res, glob L}.
+proof.
+proc*; case: (bnd{2}=t0).
+ by call rejloop_t0_eq => //.
+have ?:= dcondP_ll.
+transitivity{1}
+ { RO.init();
+   r <@ RejLoopD(RO).distinguish(bnd); }
+ ( ={bnd,glob L} /\ bnd{2} <> t0 ==> ={r, glob L} )
+ ( ={bnd,glob L} /\ bnd{2} <> t0 ==> ={r, glob L} ) => //.
++ by move=> /> &2 H; exists (glob L){2} bnd{2} => />.
++ inline RejLoop(L).loopEager RejLoopD(RO).distinguish.
+  inline RO.sample RO.get RO.init.
+  seq 4 8: (={bnd0, b, glob L} /\ bnd0{2} <> t0 /\ RO.m{2}=empty.[(bnd0{2},b{2}) <- x{1}]).
+   swap {2} 1 5.
+   seq 3 5: (={bnd0, b, glob L} /\ bnd0{2} <> t0 /\ x{1}=r1{2} /\ x3{2}=(bnd0{2},b{2})).
+    by rnd; wp; rnd; auto => /> &2 Hbnd b Hb; split; move => y; rewrite !p_llE //.
+   rcondt {2} 2.
+    by move=> &m; auto => /> *; apply mem_empty.
+   by call (: true); auto => />.
+  seq 1 1: (b{2} /\ #pre).
+   while (#pre).
+    seq 0 1: (!b{2} /\ ={bnd0, b, glob L} /\ bnd0{2} <> t0 /\ RO.m{2}=empty).
+     inline*; auto => /> &1 &2 *.
+     rewrite /rem set_valE empty_valE /= -(tomapK empty); congr.
+     by rewrite empty_valE /#.
+    seq 2 4: (#[2:]pre /\ x{1}=r2{2} /\ x4{2}=(bnd0{2},b{2})).
+     by rnd; wp; rnd; auto => /> *; split; move => y; rewrite !p_llE //.
+    rcondt {2} 1.
+     by move=> &m; auto => /> *; apply mem_empty.
+    by call (: true); auto => /> *.
+   done.
+  rcondf {2} 3.
+   by move=> &m; auto => /> *; smt(mem_set). 
+  wp; rnd{2}; auto => /> &1 &2 *; split => *.
+   smt().
+  by rewrite get_setE.
+transitivity{1}
+ { LRO.init();
+   r <@ RejLoopD(LRO).distinguish(bnd); }
+ ( ={bnd, glob L} /\ bnd{2} <> t0 ==> ={r, glob L} )
+ ( ={bnd, glob L} /\ bnd{2} <> t0 ==> ={r, glob L} ) => //.
++ by move=> /> &2 *; exists (glob L){2} bnd{2} => />.
++ call (FullEager.RO_LRO_D RejLoopD) => />.
+   move=> /> xb.
+   by case: (xb) => ? /#.
+  by inline*; auto => />.
+inline RejLoop(L).loopLazy RejLoopD(LRO).distinguish.
+inline LRO.sample LRO.get LRO.init.
+seq 6 4: (={bnd0, b, glob L} /\ bnd0{2} <> t0 /\ RO.m{1}=empty /\ b{2}).
+ while (={bnd0, b, glob L} /\ bnd0{2} <> t0 /\ RO.m{1}=empty).
+  inline *; call (: true); auto => /> &2.
+  smt(rem_id mem_empty).
+ by wp; call (: true); auto => /> *.
+rcondt {1} 3.
+ by move=> &m; auto => />; smt(mem_empty).
+by auto => /> &2 Hb *; smt(p_llE get_setE).
+qed.
+
+end section.
+
+end RejectionLoop.
+
+
+(** Instantiation of abstract theories *)
+clone import SampleEventSwap as EvSwap
+ with type in_t <- BN.t,
+      type out_t <- BN.t.
+
+clone import RejectionLoop as RSloop
+ with type t <- BN.t,
+      op p <- fun bnd x => bn x < bn bnd,
+      op t0 <- bn_ofint 0,
+      op dt <- bn_rnd
+ proof dt_ll by exact bn_rnd_ll
+ proof t0_ll by smt(bn_rnd1E bn_modulusE StdOrder.IntOrder.expr_gt0)
+ proof p_t0E by (move => *; rewrite bn_ofintK mod0z; smt(bnk_cmp))
+ proof *.
+realize p_t0P.
+move=> bnd Hbnd; rewrite bn_ofintK modz_small 1:bn_modulusE /=.
+ smt(StdOrder.IntOrder.expr_gt0).
+have ?: bn bnd <> 0 by smt(bnK).
+smt(bnk_cmp).
+qed.
+realize dtPN_ll.
+move=> bnd.
+apply (StdOrder.RealOrder.ltr_le_trans (mu1 bn_rnd bnd)).
+ rewrite bn_rnd1E. smt.
+by apply mu_le => x _ @/predC @/pred1 /= -> /#.
+qed.
+
+
+module RSampleLoop = {
+  proc loop_init(b: bool): unit = {
+    var r1, _r1;
+    Mleak.leakages <- LeakAddr [] :: Mleak.leakages;
+    r1 <@ CT_bn_rnd.JR.main(tt, witness);
+    Mleak.leakages <- LeakAddr [] :: Mleak.leakages;
+    _r1 <@ CT_bn_lt.JR.main(tt, (witness, witness));
+    Mleak.leakages <- LeakCond (!b) :: LeakAddr [] :: Mleak.leakages;
+  }
+  proc loop_body(b: bool): unit = {
+    var r1, _r1;
+    Mleak.leakages <- LeakAddr [] :: Mleak.leakages;
+    r1 <@ CT_bn_rnd.JR.main(tt, witness);
+    Mleak.leakages <- LeakAddr [] :: Mleak.leakages;
+    _r1 <@ CT_bn_lt.JR.main(tt, (witness, witness));
+    Mleak.leakages <- LeakCond (!b) :: LeakAddr [] :: Mleak.leakages;
+  }
+}.
+
+(** Main result establishes the Coupled-Composition property
+ (CC, in the PRHL_Defs terminology) for the rejection sampling.
+ The strategy  is the following:
+   1) exploit the CT property (more precisely,
+  its simpler formulation for procedures for which
+  divergence is determined by public  inputs -- CT')
+  of the called procedures (__bn_rnd and __bn_lt_cf)
+  in order to decouple the generation of leakage in
+  those functions from the relevant data;
+   2) decouple the leaked event from the generated
+  number (abstract theory EventSwap)
+   3) rearrange the samplings on the rejection loop
+  (Eager/Lazy sampling reasoning, based on the abstract
+  theory RejectionLoop).
+
+ In the between, a lot of boilerplate is needed
+ to fit the formalization on the abstract setting
+ of leakage-free definitions and related
+ meta-properties (PRHL_Defs.ec), as well
+ as instantiations required from the abstract
+ theories.                                  *)
+lemma CC_bn_rsample:
+ equiv[ CT_bn_rsample.JR.main ~ CT_bn_rsample.Meta.CC(CT_bn_rsample.JI, CT_bn_rsample.JR).main :
+  ={pin, sin, glob CT_bn_rsample.JR} ==> ={res, glob CT_bn_rsample.JR}].
+proof.
+proc*; simplify.
+inline CT_bn_rsample.Meta.CC(CT_bn_rsample.JI, CT_bn_rsample.JR).main.
+inline CT_bn_rsample.JR.main CT_bn_rsample.JI.main Mleak.__bn_rsample.
+
+transitivity {1}
+ { bnd <- pin;
+   a <- sin;
+   Mleak.leakages <- LeakAddr [] :: Mleak.leakages;
+   a <@ CT_bn_rnd.JR.main(tt,a);
+   Mleak.leakages <- LeakAddr [] :: Mleak.leakages;
+   cf <@ CT_bn_lt.JR.main(tt, (a,bnd));
+   Mleak.leakages <- LeakCond (!cf) :: LeakAddr [] :: Mleak.leakages;
+   while (!cf) {
+     Mleak.leakages <- LeakAddr [] :: Mleak.leakages;
+     a <@ CT_bn_rnd.JR.main(tt,a);
+     Mleak.leakages <- LeakAddr [] :: Mleak.leakages;
+     cf <@ CT_bn_lt.JR.main(tt, (a,bnd));
+     Mleak.leakages <- LeakCond (!cf) :: LeakAddr [] :: Mleak.leakages;
+   }
+   r <- a;
+ }
+ ( ={pin, sin, Mleak.leakages} ==> ={r, Mleak.leakages} )
+ ( ={pin, sin, Mleak.leakages} ==> ={r, Mleak.leakages} ) => //.
++ move=> /> &2 /#.
++ inline CT_bn_rnd.JR.main CT_bn_lt.JR.main.
+  wp; while(#pre /\ ={a,cf,bnd}).
+   wp; call(: ={Mleak.leakages}); first by sim.
+   by inline*; auto => />.
+  wp; call(: ={Mleak.leakages}); first by sim.
+  by inline*; auto => />.
+
+transitivity {1}
+ { bnd <- pin;
+   a <- sin;
+   Mleak.leakages <- LeakAddr [] :: Mleak.leakages;
+   a <@ CT_bn_rnd.Meta.SimR(CT_bn_rnd.JI, CT_bn_rnd.JR).main(tt,a, witness);
+   Mleak.leakages <- LeakAddr [] :: Mleak.leakages;
+   cf <@ CT_bn_lt.Meta.SimR(CT_bn_lt.JI, CT_bn_lt.JR).main(tt, (a,bnd), (witness, witness));
+   Mleak.leakages <- LeakCond (!cf) :: LeakAddr [] :: Mleak.leakages;
+   while (!cf) {
+     Mleak.leakages <- LeakAddr [] :: Mleak.leakages;
+     a <@ CT_bn_rnd.Meta.SimR(CT_bn_rnd.JI, CT_bn_rnd.JR).main(tt,a, witness);
+     Mleak.leakages <- LeakAddr [] :: Mleak.leakages;
+     cf <@ CT_bn_lt.Meta.SimR(CT_bn_lt.JI, CT_bn_lt.JR).main(tt, (a,bnd), (witness, witness));
+     Mleak.leakages <- LeakCond (!cf) :: LeakAddr [] :: Mleak.leakages;
+   }
+   r <- a;
+ }
+ ( ={pin, sin, Mleak.leakages} ==> ={r, Mleak.leakages} )
+ ( ={pin, sin, Mleak.leakages} ==> ={r, Mleak.leakages} ) => //.
++ move=> /> &2 /#.
++ wp; while(#pre /\ ={a,cf,bnd}).
+   wp; call CT'_bn_lt.
+   by wp; call CT'_bn_rnd; auto => />.
+  wp; call CT'_bn_lt.
+  by wp; call CT'_bn_rnd; auto => />.
+inline CT_bn_rnd.Meta.SimR(CT_bn_rnd.JI, CT_bn_rnd.JR).main.
+inline CT_bn_lt.Meta.SimR(CT_bn_lt.JI, CT_bn_lt.JR).main.
+swap {1} [4..5] -1.
+swap {1} [8..9] -3.
+swap {1} [11..12] -4.
+swap {1} [15..16] -6.
+
+transitivity {1}
+ { bnd <- pin;
+   a <- sin;
+   (a, cf) <@ SampleEvent.sample(bnd, (fun _ => bn_rnd), fun bnd x => bn x < bn bnd);
+   Mleak.leakages <- LeakAddr [] :: Mleak.leakages;
+   r1 <@ CT_bn_rnd.JR.main(tt, witness);
+   Mleak.leakages <- LeakAddr [] :: Mleak.leakages;
+   _r1 <@ CT_bn_lt.JR.main(tt, (witness,witness));
+   Mleak.leakages <- LeakCond (!cf) :: LeakAddr [] :: Mleak.leakages;
+   while (!cf) {
+     (a, cf) <@ SampleEvent.sample(bnd, (fun _ => bn_rnd), fun bnd x => bn x < bn bnd);
+     Mleak.leakages <- LeakAddr [] :: Mleak.leakages;
+     r1 <@ CT_bn_rnd.JR.main(tt, witness);
+     Mleak.leakages <- LeakAddr [] :: Mleak.leakages;
+     _r1 <@ CT_bn_lt.JR.main(tt, (witness,witness));
+     Mleak.leakages <- LeakCond (!cf) :: LeakAddr [] :: Mleak.leakages;
+   }
+   r <- a;
+ }
+ ( ={pin, sin, Mleak.leakages} ==> ={r, Mleak.leakages} )
+ ( ={pin, sin, Mleak.leakages} ==> ={r, Mleak.leakages} ) => //.
++ move=> /> &2 /#.
++ wp; while(#pre /\ ={a,cf,bnd}).
+   inline SampleEvent.sample.
+   swap {1} [2..3] -1.
+   swap {1} [6..7] -3.
+   swap {1} [9..10] -4.
+   swap {1} [13..14] -6.
+   wp; call(: ={Mleak.leakages}); first by sim.
+   wp; call(: ={Mleak.leakages}); first by sim.
+   inline CT_bn_lt.JI.main.
+   wp; ecall {1} (__bn_lt_cf_ph sin5.`1{1} sin5.`2{1}).
+   by inline*; auto => /> *.
+  wp; call(: ={Mleak.leakages}); first by sim.
+  wp; call(: ={Mleak.leakages}); first by sim.
+  inline CT_bn_lt.JI.main.
+  wp; ecall {1} (__bn_lt_cf_ph sin5.`1{1} sin5.`2{1}).
+  by inline*; auto => /> *.
+
+transitivity {1}
+ { bnd <- pin;
+   a <- sin;
+   (a, cf) <@ SampleEvent.sampleEv(bnd, (fun _ => bn_rnd), fun bnd x => bn x < bn bnd);
+   Mleak.leakages <- LeakAddr [] :: Mleak.leakages;
+   r1 <@ CT_bn_rnd.JR.main(tt, witness);
+   Mleak.leakages <- LeakAddr [] :: Mleak.leakages;
+   _r1 <@ CT_bn_lt.JR.main(tt, (witness,witness));
+   Mleak.leakages <- LeakCond (!cf) :: LeakAddr [] :: Mleak.leakages;
+   while (!cf) {
+     (a, cf) <@ SampleEvent.sampleEv(bnd, (fun _ => bn_rnd), fun bnd x => bn x < bn bnd);
+     Mleak.leakages <- LeakAddr [] :: Mleak.leakages;
+     r1 <@ CT_bn_rnd.JR.main(tt, witness);
+     Mleak.leakages <- LeakAddr [] :: Mleak.leakages;
+     _r1 <@ CT_bn_lt.JR.main(tt, (witness,witness));
+     Mleak.leakages <- LeakCond (!cf) :: LeakAddr [] :: Mleak.leakages;
+   }
+   r <- a;
+ }
+ ( ={pin, sin, Mleak.leakages} ==> ={r, Mleak.leakages} )
+ ( ={pin, sin, Mleak.leakages} ==> ={r, Mleak.leakages} ) => //.
++ move=> /> &2 /#.
++ wp; while(#pre /\ ={a,cf,bnd}).
+   wp; call(: ={Mleak.leakages}); first by sim.
+   wp; call(: ={Mleak.leakages}); first by sim.
+   wp; call EvSwap.sample_sampleEv.
+   by auto => />; smt(bn_rnd_ll).
+  wp; call(: ={Mleak.leakages}); first by sim.
+  wp; call(: ={Mleak.leakages}); first by sim.
+  wp; call EvSwap.sample_sampleEv.
+  by auto => />; smt(bn_rnd_ll).
+
+transitivity {1}
+ { r <@ RSloop.RejLoop(RSampleLoop).loopEager(pin); }
+ ( ={pin, sin, Mleak.leakages} ==> ={r, Mleak.leakages})
+ ( ={pin, sin, Mleak.leakages} ==> ={r, Mleak.leakages}) => //.
++ by move=> /> &2; exists Mleak.leakages{2} pin{2} sin{2} => />.
++ inline RejLoop(RSampleLoop).loopEager.
+  inline SampleEvent.sampleEv.
+  inline RSampleLoop.loop_init RSampleLoop.loop_body.
+  wp; while (={Mleak.leakages} /\ (cf,a,bnd){1}=(b,x,bnd0){2}).
+   wp; call(: ={Mleak.leakages}); first by sim.
+   wp; call(: ={Mleak.leakages}); first by sim.
+   by auto.
+  wp; call(: ={Mleak.leakages}); first by sim.
+  wp; call(: ={Mleak.leakages}); first by sim.
+  by auto.
+
+transitivity {1}
+ { r <@ RSloop.RejLoop(RSampleLoop).loopLazy(pin); }
+ ( ={pin, sin, Mleak.leakages} ==> ={r, Mleak.leakages})
+ ( ={pin, sin, Mleak.leakages} ==> ={r, Mleak.leakages}) => //.
++ by move=> /> &2; exists Mleak.leakages{2} pin{2} sin{2} => />.
++ call (rejloop_eq RSampleLoop); auto => />.
+
+inline RejLoop(RSampleLoop).loopLazy.
+inline RSampleLoop.loop_init RSampleLoop.loop_body.
+seq 9 18: (={Mleak.leakages} /\ bnd0{1}=pin2{2}).
+ transitivity {1}
+  { bnd0 <- pin;
+    (a, b) <@ SampleEvent.sampleEv(bnd0, (fun _ => bn_rnd), fun bnd x => bn x < bn bnd);
+    Mleak.leakages <- LeakAddr [] :: Mleak.leakages;
+    r10 <@ CT_bn_rnd.JR.main(tt, witness);
+    Mleak.leakages <- LeakAddr [] :: Mleak.leakages;
+    _r10 <@ CT_bn_lt.JR.main(tt, (witness, witness));
+    Mleak.leakages <- LeakCond (!b) :: LeakAddr [] :: Mleak.leakages;
+    while (!b) {
+     (a, b) <@ SampleEvent.sampleEv(bnd0, (fun _ => bn_rnd), fun bnd x => bn x < bn bnd);
+     Mleak.leakages <- LeakAddr [] :: Mleak.leakages;
+     r10 <@ CT_bn_rnd.JR.main(tt, witness);
+     Mleak.leakages <- LeakAddr [] :: Mleak.leakages;
+     _r10 <@ CT_bn_lt.JR.main(tt, (witness, witness));
+     Mleak.leakages <- LeakCond (!b) :: LeakAddr [] :: Mleak.leakages;
+    }
+   }
+   ( ={pin, sin, Mleak.leakages} ==> ={Mleak.leakages} /\ bnd0{1} = pin{2} )
+   ( ={pin, sin, Mleak.leakages} ==> ={pin, Mleak.leakages} /\ pin2{2} = pin{2} ) => //.
+ + by move => /> &2; exists Mleak.leakages{2} pin{2} sin{2} => //.
+ + inline SampleEvent.sampleEv.
+   while(#pre /\ ={b,bnd0} /\ bnd0{2} = pin{2}).
+    wp; call(: ={Mleak.leakages}); first by sim.
+    wp; call(: ={Mleak.leakages}); first by sim.
+    by wp; rnd{2}; auto => /> &2 b b'; smt(dbiased_dcond_ll bn_rnd_ll).
+   wp; call(: ={Mleak.leakages}); first by sim.
+   wp; call(: ={Mleak.leakages}); first by sim.
+   by wp; rnd{2}; auto => /> &2 b b';  smt(dbiased_dcond_ll bn_rnd_ll).
+
+ transitivity {1}
+  { bnd0 <- pin;
+    (a, b) <@ SampleEvent.sample(bnd0, (fun _ => bn_rnd), fun bnd x => bn x < bn bnd);
+    Mleak.leakages <- LeakAddr [] :: Mleak.leakages;
+    r10 <@ CT_bn_rnd.JR.main(tt, witness);
+    Mleak.leakages <- LeakAddr [] :: Mleak.leakages;
+    _r10 <@ CT_bn_lt.JR.main(tt, (witness, witness));
+    Mleak.leakages <- LeakCond (!b) :: LeakAddr [] :: Mleak.leakages;
+    while (!b) {
+     (a, b) <@ SampleEvent.sample(bnd0, (fun _ => bn_rnd), fun bnd x => bn x < bn bnd);
+     Mleak.leakages <- LeakAddr [] :: Mleak.leakages;
+     r10 <@ CT_bn_rnd.JR.main(tt, witness);
+     Mleak.leakages <- LeakAddr [] :: Mleak.leakages;
+     _r10 <@ CT_bn_lt.JR.main(tt, (witness, witness));
+     Mleak.leakages <- LeakCond (!b) :: LeakAddr [] :: Mleak.leakages;
+    }
+   }
+   ( ={pin, sin, Mleak.leakages} ==> ={pin, Mleak.leakages} /\ bnd0{1} = pin{2} )
+   ( ={pin, sin, Mleak.leakages} ==> ={pin, Mleak.leakages} /\ pin2{2}=pin{2} ) => //.
+ + by move => /> &2; exists Mleak.leakages{2} pin{2} sin{2} => //.
+ + symmetry. 
+   while(#pre /\ ={b,bnd0} /\ bnd0{2} = pin{2}).
+    wp; call(: ={Mleak.leakages}); first by sim.
+    wp; call(: ={Mleak.leakages}); first by sim.
+    wp; call EvSwap.sample_sampleEv.
+    auto => />; smt(bn_rnd_ll).
+   wp; call(: ={Mleak.leakages}); first by sim.
+   wp; call(: ={Mleak.leakages}); first by sim.
+   wp; call EvSwap.sample_sampleEv.
+   by auto => />; smt(bn_rnd_ll).
+ inline SampleEvent.sample.
+ transitivity {2}
+  { Mleak.leakages <- LeakAddr [] :: Mleak.leakages;
+    a <@ CT_bn_rnd.JR.main(tt,sin);
+    Mleak.leakages <- LeakAddr [] :: Mleak.leakages;
+    cf <@ CT_bn_lt.JR.main(tt, (a,pin));
+    Mleak.leakages <- LeakCond (!cf) :: LeakAddr [] :: Mleak.leakages;
+    while (!cf) {
+     Mleak.leakages <- LeakAddr [] :: Mleak.leakages;
+     a <@ CT_bn_rnd.JR.main(tt,sin);
+     Mleak.leakages <- LeakAddr [] :: Mleak.leakages;
+     cf <@ CT_bn_lt.JR.main(tt, (a,pin));
+     Mleak.leakages <- LeakCond (!cf) :: LeakAddr [] :: Mleak.leakages;
+    }
+   }
+   ( ={pin, sin, Mleak.leakages} ==> ={pin, Mleak.leakages} /\ bnd0{1} = pin{2} )
+   ( ={pin, sin, Mleak.leakages} ==> ={pin, Mleak.leakages} /\ pin2{2} = pin{2} ) => //.
+ + by move => /> &2; exists Mleak.leakages{2} pin{2} sin{2} => //.
+ + transitivity {2}
+    { Mleak.leakages <- LeakAddr [] :: Mleak.leakages;
+      a <@ CT_bn_rnd.Meta.SimR(CT_bn_rnd.JI, CT_bn_rnd.JR).main(tt,sin,witness);
+      Mleak.leakages <- LeakAddr [] :: Mleak.leakages;
+      cf <@ CT_bn_lt.Meta.SimR(CT_bn_lt.JI, CT_bn_lt.JR).main(tt, (a,pin), (witness,witness));
+      Mleak.leakages <- LeakCond (!cf) :: LeakAddr [] :: Mleak.leakages;
+      while (!cf) {
+       Mleak.leakages <- LeakAddr [] :: Mleak.leakages;
+       a <@ CT_bn_rnd.Meta.SimR(CT_bn_rnd.JI, CT_bn_rnd.JR).main(tt,sin,witness);
+       Mleak.leakages <- LeakAddr [] :: Mleak.leakages;
+       cf <@ CT_bn_lt.Meta.SimR(CT_bn_lt.JI, CT_bn_lt.JR).main(tt, (a,pin), (witness,witness));
+       Mleak.leakages <- LeakCond (!cf) :: LeakAddr [] :: Mleak.leakages;
+      }
+     }
+     ( ={pin, sin, Mleak.leakages} ==> ={pin, Mleak.leakages} /\ bnd0{1} = pin{2} )
+     ( ={pin, sin, Mleak.leakages} ==> ={pin, Mleak.leakages} ) => //.
+   - by move => /> &2; exists Mleak.leakages{2} pin{2} sin{2} => //.
+   - inline CT_bn_rnd.Meta.SimR CT_bn_lt.Meta.SimR.
+     inline CT_bn_rnd.JI.main CT_bn_lt.JI.main.
+     while ((b,bnd0){1}=(cf,pin){2} /\ ={Mleak.leakages} ).
+      swap {2} [7..10] -3.
+      swap {2} [16..20] -2.
+      swap {2} [12..18] -3.
+      swap {2} 1 14.
+      wp; call(: ={Mleak.leakages}); first by sim.
+      wp; call(: ={Mleak.leakages}); first by sim.
+      wp; ecall {2} (__bn_lt_cf_ph sin10{2}.`1 sin10{2}.`2).
+      by inline*; auto => />.
+     swap {2} [6..10] -2.
+     swap {2} [16..20] -2.
+     swap {2} [12..18] -3.
+     swap {2} 1 14.
+     wp; call(: ={Mleak.leakages}); first by sim.
+     wp; call(: ={Mleak.leakages}); first by sim.
+     wp; ecall {2} (__bn_lt_cf_ph sin8{2}.`1 sin8{2}.`2).
+     by inline*; auto => /> *.
+   symmetry.
+   while (#pre /\ ={cf}).
+    wp; call CT'_bn_lt.
+    by wp; call CT'_bn_rnd; auto.
+   wp; call CT'_bn_lt.
+   by wp; call CT'_bn_rnd; auto.
+ inline CT_bn_rnd.JR.main CT_bn_lt.JR.main.
+ wp; while(#pre /\ ={a,cf} /\ bnd{2}=pin{2}).
+  wp; call(: ={Mleak.leakages}); first by sim.
+  by inline*; auto => />.
+ wp; call(: ={Mleak.leakages}); first by sim.
+ by inline*; auto => />.
+wp.
+transitivity {2}
+ { r2 <@ M.bn_sample_bnd(sin2,pin2); }
+ ( ={Mleak.leakages} /\ bnd0{1} = pin2{2} ==> x{1} = r2{2} /\ ={Mleak.leakages} )
+ ( ={pin2,Mleak.leakages} ==> ={r2, Mleak.leakages}) => //.
++ by move=> /> &2; exists Mleak.leakages{2} pin2{2}.
++ inline*; wp.
+  rnd (bnk nlimbs) bn_ofint.
+  auto => /> &2; split.
+   move=> x; rewrite supp_dinter => Hx.
+   rewrite bn_ofintK modz_small; smt(bnk_cmp).
+  move => H1; split.
+   move=> x; rewrite supp_dinter => Hx.
+   rewrite -bn_rnd_bndE /bn_rnd_bnd dmap1E.
+   apply mu_eq_support => y.
+   rewrite supp_dinter => Hy.
+   rewrite /pred1 /(\o) /= eq_iff => *; split => // E.
+   rewrite (:y=y%%bn_modulus) 1:modz_small //; first smt(bnk_cmp). 
+   rewrite (:x=x%%bn_modulus) 1:modz_small //; first smt(bnk_cmp). 
+   by rewrite -!bn_ofintK E.
+  move=> H2 x; rewrite dcond_supp /= => [[H3 H4]].
+  rewrite supp_dinter; smt(bnk_cmp bnK).
+
+by symmetry; call __bn_rsample_eq; auto => />.
+qed.
+
+(** The actual CT property follows from a generic
+ property formalised in PRHL_Defs.        *)
+lemma CT_bn_rsample:
+ equiv[  CT_bn_rsample.Meta.RSim(CT_bn_rsample.JI, CT_bn_rsample.JR).main ~  CT_bn_rsample.Meta.SimR(CT_bn_rsample.JI, CT_bn_rsample.JR).main :
+  ={pin, sin, glob CT_bn_rsample.JR} ==> ={res, glob CT_bn_rsample.JR}].
+proof.
+print CT_bn_rsample.Meta.
+apply (CT_bn_rsample.Meta.pinll_ct_CC_CT CT_bn_rsample.JR CT_bn_rsample.JI).
++ by apply CT_bn_rsample.stateless_JI.
++ by apply CT_bn_rsample.proj_JR_JI.
++ by apply CT_bn_rsample.prMuE.
++ exists (fun bnd => bn bnd <> 0) => /> _bnd.
+  case: (bn _bnd=0) => C /=; proc; simplify.
+   hoare; inline M.__bn_rsample.
+   wp; while(bnd=_bnd /\ cf = bnk nlimbs a < bnk nlimbs _bnd).
+    ecall (__bn_lt_cf_h a bnd).
+    by inline*; auto => /> &m.
+   ecall (__bn_lt_cf_h a bnd).
+   by inline*; auto => &m -> a Ha r;  smt(bnk_cmp).
+  call (__bn_rsample_ll); auto => />.
+  smt(bnk_cmp).
+split.
+ proc.
+ by ecall (__bn_rsample_ct).
+by apply CC_bn_rsample.
+qed.
+
+
+end BN_base.
+
